@prefix a-popis-dat-pojem: <http://onto.fel.cvut.cz/ontologies/slovník/agendový/popis-dat/pojem/> .
@prefix dcterms: <http://purl.org/dc/terms/> .
@prefix g-sgov-iso-iec-27034-12011-11-15: <https://slovník.gov.cz/generický/iso-iec-27034-12011-11-15/> .
@prefix g-sgov-iso-iec-27034-12011-11-15-pojem: <https://slovník.gov.cz/generický/iso-iec-27034-12011-11-15/pojem/> .
@prefix rdf: <http://www.w3.org/1999/02/22-rdf-syntax-ns#> .
@prefix skos: <http://www.w3.org/2004/02/skos/core#> .
@prefix xsd: <http://www.w3.org/2001/XMLSchema#> .

g-sgov-iso-iec-27034-12011-11-15:glosář a a-popis-dat-pojem:glosář, skos:ConceptScheme;
  dcterms:title "ISO/IEC 27034-1:2011-11-15"@cs;
  skos:hasTopConcept g-sgov-iso-iec-27034-12011-11-15-pojem:model-životního-cyklu, g-sgov-iso-iec-27034-12011-11-15-pojem:operační-prostředí,
    g-sgov-iso-iec-27034-12011-11-15-pojem:produkt, g-sgov-iso-iec-27034-12011-11-15-pojem:údržba,
    g-sgov-iso-iec-27034-12011-11-15-pojem:řízení-bezpečnosti-aplikace, g-sgov-iso-iec-27034-12011-11-15-pojem:životní-cyklus .

g-sgov-iso-iec-27034-12011-11-15-pojem:model-životního-cyklu a skos:Concept;
  dcterms:source "3.14";
  skos:definition """framework of processes and activities concerned with the life cycle that may be organized into stages, which also acts as a common reference for communication and understanding
[SOURCE: ISO/IEC 12207:2008, definition 4.17]"""@en;
  skos:inScheme g-sgov-iso-iec-27034-12011-11-15:glosář;
  skos:prefLabel "Life Cycle Model"@en, "Model životního cyklu"@cs .

g-sgov-iso-iec-27034-12011-11-15-pojem:operační-prostředí a skos:Concept;
  dcterms:source "3.18";
  skos:definition """external surroundings of a program existing or expected to exist during its execution
[SOURCE: ISO/IEC 2382-7:2000, definition 07.11.07]"""@en;
  skos:inScheme g-sgov-iso-iec-27034-12011-11-15:glosář;
  skos:prefLabel "Operating Environment"@en, "Operační prostředí"@cs .

g-sgov-iso-iec-27034-12011-11-15-pojem:produkt a skos:Concept;
  dcterms:source "3.19";
  skos:definition """result of a process
[SOURCE: ISO 9000:2005, definition 3.4.2]"""@en;
  skos:inScheme g-sgov-iso-iec-27034-12011-11-15:glosář;
  skos:prefLabel "Product"@en, "Produkt"@cs .

g-sgov-iso-iec-27034-12011-11-15-pojem:údržba a skos:Concept;
  dcterms:source "3.15";
  skos:definition """any change performed on an application after its delivery
EXAMPLES　Error correction, added functionality, improved performance, ensuring the application's functionality."""@en;
  skos:inScheme g-sgov-iso-iec-27034-12011-11-15:glosář;
  skos:prefLabel "Maintenance"@en, "Údržba"@cs .

g-sgov-iso-iec-27034-12011-11-15-pojem:řízení-bezpečnosti-aplikace a skos:Concept;
  dcterms:source "3.8";
  skos:definition "data structure containing a precise enumeration and description of a security activity and its associated verification measurement to be performed at a specific point in an application's life cycle"@en;
  skos:inScheme g-sgov-iso-iec-27034-12011-11-15:glosář;
  skos:prefLabel "Application Security Control"@en, "Řízení bezpečnosti aplikace"@cs .

g-sgov-iso-iec-27034-12011-11-15-pojem:životní-cyklus a skos:Concept;
  dcterms:source "3.13";
  skos:definition """evolution of a system, product, service, project or other human-made entity from conception through retirement
[SOURCE: ISO/IEC 12207:2008, definition 4.16]
A term used to refer to the stages (or just the duration) of things that have a beginning and an end — changing form (maturing, usually) along the way from concept; expanded into a set of requirements; to transition, then deployment, and finally retirement.."""@en;
  skos:inScheme g-sgov-iso-iec-27034-12011-11-15:glosář;
  skos:prefLabel "Life Cycle"@en, "Životní cyklus"@cs .
