@prefix a-popis-dat-pojem: <http://onto.fel.cvut.cz/ontologies/slovník/agendový/popis-dat/pojem/> .
@prefix dcterms: <http://purl.org/dc/terms/> .
@prefix g-sgov-iso-iec-tr-270192013-07-15: <https://slovník.gov.cz/generický/iso-iec-tr-270192013-07-15/> .
@prefix g-sgov-iso-iec-tr-270192013-07-15-pojem: <https://slovník.gov.cz/generický/iso-iec-tr-270192013-07-15/pojem/> .
@prefix rdf: <http://www.w3.org/1999/02/22-rdf-syntax-ns#> .
@prefix skos: <http://www.w3.org/2004/02/skos/core#> .
@prefix xsd: <http://www.w3.org/2001/XMLSchema#> .

g-sgov-iso-iec-tr-270192013-07-15:glosář a a-popis-dat-pojem:glosář, skos:ConceptScheme;
  dcterms:title "ISO/IEC TR 27019:2013-07-15"@cs;
  skos:hasTopConcept g-sgov-iso-iec-tr-270192013-07-15-pojem:blackout, g-sgov-iso-iec-tr-270192013-07-15-pojem:dohledové-centrum,
    g-sgov-iso-iec-tr-270192013-07-15-pojem:kritická-infrastruktura, g-sgov-iso-iec-tr-270192013-07-15-pojem:prohlášení-o-použitelnosti,
    g-sgov-iso-iec-tr-270192013-07-15-pojem:systém-řízení-procesů .

g-sgov-iso-iec-tr-270192013-07-15-pojem:blackout a skos:Concept;
  dcterms:source "3.1";
  skos:definition "widespread electrical power outage"@en;
  skos:inScheme g-sgov-iso-iec-tr-270192013-07-15:glosář;
  skos:prefLabel "Blackout"@cs, "Blackout"@en .

g-sgov-iso-iec-tr-270192013-07-15-pojem:dohledové-centrum a skos:Concept;
  dcterms:source "3.2";
  skos:definition "team of security experts to support the handling of information security incidents"@en,
    "tým bezpečnostních expertů na podporu řešení incidentů informační bezpečnosti "@cs;
  skos:inScheme g-sgov-iso-iec-tr-270192013-07-15:glosář;
  skos:prefLabel "Computer Emergency Response Team"@en, "Dohledové centrum "@cs .

g-sgov-iso-iec-tr-270192013-07-15-pojem:kritická-infrastruktura a skos:Concept;
  dcterms:source "3.3";
  skos:definition "organizations and facilities that are essential for the functioning of society and the economy as a whole NOTE　A failure or malfunction of such organizations and facilities would result in sustained supply shortfalls, make a significant impact on public security and have other wide ranging impacts."@en;
  skos:inScheme g-sgov-iso-iec-tr-270192013-07-15:glosář;
  skos:prefLabel "Critical infrastructure"@en, "Kritická infrastruktura"@cs .

g-sgov-iso-iec-tr-270192013-07-15-pojem:prohlášení-o-použitelnosti a skos:Concept;
  dcterms:source "3.16";
  skos:definition "Documented statement describing the control objectives and controls that are relevant and applicable to the organization’s ISMS"@en;
  skos:inScheme g-sgov-iso-iec-tr-270192013-07-15:glosář;
  skos:prefLabel "Prohlášení o použitelnosti"@cs, "Statement of Applicability"@en .

g-sgov-iso-iec-tr-270192013-07-15-pojem:systém-řízení-procesů a skos:Concept;
  dcterms:source "3.12";
  skos:definition "system that serves to control and monitor the generation, transmission, storage and distribution of electric power, gas and heat in combination with the control of supporting processes"@en;
  skos:inScheme g-sgov-iso-iec-tr-270192013-07-15:glosář;
  skos:prefLabel "Process Control Systém"@en, "Systém řízení procesů"@cs .
