@prefix a-popis-dat-pojem: <http://onto.fel.cvut.cz/ontologies/slovník/agendový/popis-dat/pojem/> .
@prefix dcterms: <http://purl.org/dc/terms/> .
@prefix g-sgov-iso-iec-270002016-02-15: <https://slovník.gov.cz/generický/iso-iec-270002016-02-15/> .
@prefix g-sgov-iso-iec-270002016-02-15-pojem: <https://slovník.gov.cz/generický/iso-iec-270002016-02-15/pojem/> .
@prefix rdf: <http://www.w3.org/1999/02/22-rdf-syntax-ns#> .
@prefix skos: <http://www.w3.org/2004/02/skos/core#> .
@prefix xsd: <http://www.w3.org/2001/XMLSchema#> .

g-sgov-iso-iec-270002016-02-15:glosář a a-popis-dat-pojem:glosář, skos:ConceptScheme;
  dcterms:title "ISO/IEC 27000:2016-02-15"@cs;
  skos:hasTopConcept g-sgov-iso-iec-270002016-02-15-pojem:bezpečnost-informací, g-sgov-iso-iec-270002016-02-15-pojem:hrozba,
    g-sgov-iso-iec-270002016-02-15-pojem:informační-systém, g-sgov-iso-iec-270002016-02-15-pojem:kompetence,
    g-sgov-iso-iec-270002016-02-15-pojem:metrika, g-sgov-iso-iec-270002016-02-15-pojem:následek---dopad,
    g-sgov-iso-iec-270002016-02-15-pojem:objekt, g-sgov-iso-iec-270002016-02-15-pojem:ověření,
    g-sgov-iso-iec-270002016-02-15-pojem:posouzení, g-sgov-iso-iec-270002016-02-15-pojem:proces,
    g-sgov-iso-iec-270002016-02-15-pojem:proces-řízení-rizik, g-sgov-iso-iec-270002016-02-15-pojem:riziko,
    g-sgov-iso-iec-270002016-02-15-pojem:vrcholový-management, g-sgov-iso-iec-270002016-02-15-pojem:výkon,
    g-sgov-iso-iec-270002016-02-15-pojem:výkoný-management, g-sgov-iso-iec-270002016-02-15-pojem:zainteresovaný,
    g-sgov-iso-iec-270002016-02-15-pojem:zbytková-rizika, g-sgov-iso-iec-270002016-02-15-pojem:řízení,
    g-sgov-iso-iec-270002016-02-15-pojem:řízení-přístupů .

g-sgov-iso-iec-270002016-02-15-pojem:bezpečnost-informací a skos:Concept;
  dcterms:source "2.33";
  skos:definition """preservation of confidentiality (2.12), integrity (2.40) and availability (2.9) of information
Note 1 to entry: In addition, other properties, such as authenticity (2.8), accountability, non-repudiation (2.54), and reliability (2.62) can also be involved."""@en;
  skos:inScheme g-sgov-iso-iec-270002016-02-15:glosář;
  skos:prefLabel "Bezpečnost informací"@cs, "Information security"@en .

g-sgov-iso-iec-270002016-02-15-pojem:hrozba a skos:Concept;
  dcterms:source "2.83";
  skos:definition "potential cause of an unwanted incident, which may result in harm to a system or organization (2.57)"@en;
  skos:inScheme g-sgov-iso-iec-270002016-02-15:glosář;
  skos:prefLabel "Hrozba"@cs, "Threat"@en .

g-sgov-iso-iec-270002016-02-15-pojem:informační-systém a skos:Concept;
  dcterms:source "2.39";
  skos:definition "applications, services, information technology assets, or other information handling components"@en;
  skos:inScheme g-sgov-iso-iec-270002016-02-15:glosář;
  skos:prefLabel "Information system"@en, "Informační systém"@cs .

g-sgov-iso-iec-270002016-02-15-pojem:kompetence a skos:Concept;
  dcterms:source "2.11";
  skos:definition "Schopnost aplikovat znalosti a dovednosti k dosažení určeného výsledku."@cs,
    "ability to apply knowledge and skills to achieve intended results"@en;
  skos:inScheme g-sgov-iso-iec-270002016-02-15:glosář;
  skos:prefLabel "Competence"@en, "Kompetence"@cs .

g-sgov-iso-iec-270002016-02-15-pojem:metrika a skos:Concept;
  dcterms:source "2.48";
  skos:definition "proces určování hodnoty"@cs, """process (2.61) to determine a value
Note 1 to entry: In the context of information security (2.33), the process (2.61) of determining a value requires information about the effectiveness (2.24) of an information security (2.33) management system (2.46) and its associated controls (2.16) using a measurement method (2.50), a measurement function (2.49), an analytical model (2.2), and decision criteria (2.21)."""@en;
  skos:inScheme g-sgov-iso-iec-270002016-02-15:glosář;
  skos:prefLabel "Measurement"@en, "Metrika"@cs .

g-sgov-iso-iec-270002016-02-15-pojem:následek---dopad a skos:Concept;
  dcterms:source "2.14";
  skos:definition """outcome of an event (2.25) affecting objectives (2.56)
[SOURCE: ISO Guide 73:2009, 3.6.1.3, modified]
Note 1 to entry: An event (2.25) can lead to a range of consequences.
Note 2 to entry: A consequence can be certain or uncertain and in the context of information security (2.33) is usually negative.
Note 3 to entry: Consequences can be expressed qualitatively or quantitatively.
Note 4 to entry: Initial consequences can escalate through knock-on effects."""@en;
  skos:inScheme g-sgov-iso-iec-270002016-02-15:glosář;
  skos:prefLabel "Consequence"@en, "Následek / dopad"@cs .

g-sgov-iso-iec-270002016-02-15-pojem:objekt a skos:Concept;
  dcterms:source "2.55";
  skos:definition "item characterized through the measurement (2.48) of its attributes (2.4)"@en;
  skos:inScheme g-sgov-iso-iec-270002016-02-15:glosář;
  skos:prefLabel "Object"@en, "Objekt"@cs .

g-sgov-iso-iec-270002016-02-15-pojem:ověření a skos:Concept;
  dcterms:source "2.87";
  skos:definition """confirmation, through the provision of objective evidence, that the requirements (2.63) for a specific intended use or application have been fulfilled
[SOURCE: ISO 9000:2015, 3.8.12, modified]"""@en;
  skos:inScheme g-sgov-iso-iec-270002016-02-15:glosář;
  skos:prefLabel "Ověření"@cs, "validation"@en .

g-sgov-iso-iec-270002016-02-15-pojem:posouzení a skos:Concept;
  dcterms:source "2.65";
  skos:definition """activity undertaken to determine the suitability, adequacy and effectiveness (2.24) of the subject matter to achieve established objectives (2.54)
[SOURCE: ISO Guide 73:2009, 3.8.2.2, modified — Note 1 to entry has been deleted.]"""@en;
  skos:inScheme g-sgov-iso-iec-270002016-02-15:glosář;
  skos:prefLabel "Posouzení"@cs, "Review"@en .

g-sgov-iso-iec-270002016-02-15-pojem:proces a skos:Concept;
  dcterms:source "2.61";
  skos:definition "set of interrelated or interacting activities which transforms inputs into outputs"@en;
  skos:inScheme g-sgov-iso-iec-270002016-02-15:glosář;
  skos:prefLabel "Proces"@cs, "Process"@en .

g-sgov-iso-iec-270002016-02-15-pojem:proces-řízení-rizik a skos:Concept;
  dcterms:source "2.77";
  skos:definition """systematic application of management policies (2.60), procedures and practices to the activities of communicating, consulting, establishing the context and identifying,  analysing, evaluating, treating, monitoring and reviewing risk (2.68)
[SOURCE: ISO Guide 73:2009, 3.1, modified — Note 1 to entry has been added.]
Note 1 to entry: ISO/IEC 27005 uses the term “process” (2.61) to describe risk management overall. The elements within the risk management (2.76) process (2.61) are termed “activities”."""@en;
  skos:inScheme g-sgov-iso-iec-270002016-02-15:glosář;
  skos:prefLabel "Proces řízení rizik"@cs, "Risk Management Process"@en .

g-sgov-iso-iec-270002016-02-15-pojem:riziko a skos:Concept;
  dcterms:source "2.68";
  skos:definition """effect of uncertainty on objectives
[SOURCE: ISO Guide 73:2009, 1.1, modified]
Note 1 to entry: An effect is a deviation from the expected — positive or negative.
Note 2 to entry: Uncertainty is the state, even partial, of deficiency of information related to, understanding or knowledge of, an event (2.25), its consequence (2.14), or likelihood (2.45).
Note 3 to entry: Risk is often characterized by reference to potential events (2.25) and consequences (2.14), or a combination of these.
Note 4 to entry: Risk is often expressed in terms of a combination of the consequences (2.14) of an event (2.25) (including changes in circumstances) and the associated likelihood (2.45) of occurrence.
Note 5 to entry: In the context of information security (2.33) management systems (2.46), information security (2.33) risks can be expressed as effect of uncertainty on information security (2.33) objectives (2.56).
Note 6 to entry: Information security (2.33) risk is associated with the potential that threats (2.83) will exploit vulnerabilities (2.89) of an information asset or group of information assets and thereby cause harm to an organization (2.57)."""@en;
  skos:inScheme g-sgov-iso-iec-270002016-02-15:glosář;
  skos:prefLabel "Risk"@en, "Riziko"@cs .

g-sgov-iso-iec-270002016-02-15-pojem:vrcholový-management a skos:Concept;
  dcterms:source "2.84";
  skos:definition """person or group of people who directs and controls an organization (2.57) at the highest level
Note 1 to entry: Top management has the power to delegate authority and provide resources within the organization (2.57).
Note 2 to entry: If the scope of the management system (2.46) covers only part of an organization (2.57), then top management refers to those who direct and control that part of the organization (2.57)."""@en;
  skos:inScheme g-sgov-iso-iec-270002016-02-15:glosář;
  skos:prefLabel "Top Management"@en, "Vrcholový management"@cs .

g-sgov-iso-iec-270002016-02-15-pojem:výkon a skos:Concept;
  dcterms:source "2.59";
  skos:definition """measurable result
Note 1 to entry: Performance can relate either to quantitative or qualitative findings.
Note 2 to entry: Performance can relate to the management of activities, processes (2.61), products (including services), systems or organizations (2.57)."""@en;
  skos:inScheme g-sgov-iso-iec-270002016-02-15:glosář;
  skos:prefLabel "Performance"@en, "Výkon"@cs .

g-sgov-iso-iec-270002016-02-15-pojem:výkoný-management a skos:Concept;
  dcterms:source "2.26";
  skos:definition """person or group of people who have delegated responsibility from the governing body (2.29) for implementation of strategies and policies to accomplish the purpose of the organization (2.57)
Note 1 to entry: Executive management is sometimes called top management (2.84) and can include Chief Executive Officers, Chief Financial Officers, Chief Information Officers, and similar roles."""@en;
  skos:inScheme g-sgov-iso-iec-270002016-02-15:glosář;
  skos:prefLabel "Executive Management"@en, "Výkoný management"@cs .

g-sgov-iso-iec-270002016-02-15-pojem:zainteresovaný a skos:Concept;
  dcterms:source "2.82";
  skos:definition """person or organization (2.57) that can affect, be affected by, or perceive themselves to be affected by a decision or activity
[SOURCE: ISO Guide 73:2009, 3.2.1.1, modified — Note 1 to entry has been deleted.]"""@en;
  skos:inScheme g-sgov-iso-iec-270002016-02-15:glosář;
  skos:prefLabel "Stakeholder"@en, "Zainteresovaný"@cs .

g-sgov-iso-iec-270002016-02-15-pojem:zbytková-rizika a skos:Concept;
  dcterms:source "2.64";
  skos:definition """risk (2.68) remaining after risk treatment (2.79)
Note 1 to entry: Residual risk can contain unidentified risk (2.68).
Note 2 to entry: Residual risk can also be known as “retained risk”."""@en;
  skos:inScheme g-sgov-iso-iec-270002016-02-15:glosář;
  skos:prefLabel "Residual Risk"@en, "Zbytková rizika"@cs .

g-sgov-iso-iec-270002016-02-15-pojem:řízení a skos:Concept;
  dcterms:source "2.16";
  skos:definition """measure that is modifying risk (2.68)
[SOURCE: ISO Guide 73:2009, 3.8.1.1]
Note 1 to entry: Controls include any process (2.61), policy (2.60), device, practice, or other actions which modify risk (2.68).
Note 2 to entry: Controls may not always exert the intended or assumed modifying effect."""@en;
  skos:inScheme g-sgov-iso-iec-270002016-02-15:glosář;
  skos:prefLabel "Control"@en, "Řízení"@cs .

g-sgov-iso-iec-270002016-02-15-pojem:řízení-přístupů a skos:Concept;
  dcterms:source "2.1";
  skos:definition "means to ensure that access to assets is authorized and restricted based on business and security requirements (2.63)"@en;
  skos:inScheme g-sgov-iso-iec-270002016-02-15:glosář;
  skos:prefLabel "Access control"@en, "Řízení přístupů"@cs .
