@prefix a-popis-dat-pojem: <http://onto.fel.cvut.cz/ontologies/slovník/agendový/popis-dat/pojem/> .
@prefix dcterms: <http://purl.org/dc/terms/> .
@prefix g-sgov-iso-iec-270402015-01-15: <https://slovník.gov.cz/generický/iso-iec-270402015-01-15/> .
@prefix g-sgov-iso-iec-270402015-01-15-pojem: <https://slovník.gov.cz/generický/iso-iec-270402015-01-15/pojem/> .
@prefix rdf: <http://www.w3.org/1999/02/22-rdf-syntax-ns#> .
@prefix skos: <http://www.w3.org/2004/02/skos/core#> .
@prefix xsd: <http://www.w3.org/2001/XMLSchema#> .

g-sgov-iso-iec-270402015-01-15:glosář a a-popis-dat-pojem:glosář, skos:ConceptScheme;
  dcterms:title "ISO/IEC 27040:2015-01-15"@cs;
  skos:hasTopConcept g-sgov-iso-iec-270402015-01-15-pojem:cílová-data, g-sgov-iso-iec-270402015-01-15-pojem:elektronicky-uložené-informace,
    g-sgov-iso-iec-270402015-01-15-pojem:gateway, g-sgov-iso-iec-270402015-01-15-pojem:jediný-bod-selhání,
    g-sgov-iso-iec-270402015-01-15-pojem:komprese, g-sgov-iso-iec-270402015-01-15-pojem:metadata,
    g-sgov-iso-iec-270402015-01-15-pojem:paměťové-médium, g-sgov-iso-iec-270402015-01-15-pojem:paměťové-zařízení .

g-sgov-iso-iec-270402015-01-15-pojem:cílová-data a skos:Concept;
  dcterms:source "3.52";
  skos:definition "information subject to a given process, typically including most or all information on a piece of storage media (3.48)"@en;
  skos:inScheme g-sgov-iso-iec-270402015-01-15:glosář;
  skos:prefLabel "Cílová data"@cs, "target data"@en .

g-sgov-iso-iec-270402015-01-15-pojem:elektronicky-uložené-informace a skos:Concept;
  dcterms:source "3.16";
  skos:definition """data or information of any kind and from any source, whose temporal existence is evidenced by being stored (3.50) in, or on, any electronic medium
Note 1 to entry: Electronically Stored Information (ESI) includes traditional e-mail, memos, letters, spreadsheets, databases, office documents, presentations, and other  electronic formats commonly found on a computer. ESI also includes system, application, and file-associated metadata (3.26) such as timestamps, revision history, file type, etc.
Note 2 to entry: Electronic medium can take the form of, but is not limited to, storage devices (3.45) and storage elements (3.47)."""@en;
  skos:inScheme g-sgov-iso-iec-270402015-01-15:glosář;
  skos:prefLabel "Electronically Stored Information"@en, "Elektronicky uložené informace"@cs .

g-sgov-iso-iec-270402015-01-15-pojem:gateway a skos:Concept;
  dcterms:source "3.19";
  skos:definition "device (3.14) that converts a protocol to another protocol"@en;
  skos:inScheme g-sgov-iso-iec-270402015-01-15:glosář;
  skos:prefLabel "Gateway"@cs, "Gateway"@en .

g-sgov-iso-iec-270402015-01-15-pojem:jediný-bod-selhání a skos:Concept;
  dcterms:source "3.42";
  skos:definition """element or component of a system, a path in a system, or a system that, if it fails, the whole system or an array of systems are unable to perform their primary functions
Note 1 to entry: A single point of failure is often considered a design flaw associated with a critical element."""@en;
  skos:inScheme g-sgov-iso-iec-270402015-01-15:glosář;
  skos:prefLabel "Jediný bod selhání"@cs, "Single Point of Failure"@en .

g-sgov-iso-iec-270402015-01-15-pojem:komprese a skos:Concept;
  dcterms:source "3.3";
  skos:definition """process of removing redundancies in digital data to reduce the amount that should be stored (3.50) or transmitted
[SOURCE: ISO/TR 12033:2009, 3.1]
Note 1 to entry: For storage (3.43), lossless compression (i.e., compression using a technique that preserves the entire content of the original data, and from which the  original data can be reconstructed exactly) is required."""@en;
  skos:inScheme g-sgov-iso-iec-270402015-01-15:glosář;
  skos:prefLabel "Compression"@en, "Komprese"@cs .

g-sgov-iso-iec-270402015-01-15-pojem:metadata a skos:Concept;
  dcterms:source "3.26";
  skos:definition "data that define and describe other data [SOURCE: ISO/IEC 11179 1:2004, 3.2.16]"@en;
  skos:inScheme g-sgov-iso-iec-270402015-01-15:glosář;
  skos:prefLabel "Metadata"@cs, "Metadata"@en .

g-sgov-iso-iec-270402015-01-15-pojem:paměťové-médium a skos:Concept;
  dcterms:source "3.48";
  skos:definition "material on which Electronically Stored Information (3.16) or digital data are or can be recorded"@en;
  skos:inScheme g-sgov-iso-iec-270402015-01-15:glosář;
  skos:prefLabel "Paměťové médium"@cs, "Storage Medium / Storage Media"@en .

g-sgov-iso-iec-270402015-01-15-pojem:paměťové-zařízení a skos:Concept;
  dcterms:source "3.45";
  skos:definition "any storage element (3.48) or aggregation of storage elements (3.47), designed and built primarily for the purpose of data storage (3.43) and delivery"@en;
  skos:inScheme g-sgov-iso-iec-270402015-01-15:glosář;
  skos:prefLabel "Paměťové zařízení"@cs, "Storage Device"@en .
