@prefix a-popis-dat-pojem: <http://onto.fel.cvut.cz/ontologies/slovník/agendový/popis-dat/pojem/> .
@prefix dcterms: <http://purl.org/dc/terms/> .
@prefix g-sgov-iso-iec-270312011-03-01: <https://slovník.gov.cz/generický/iso-iec-270312011-03-01/> .
@prefix g-sgov-iso-iec-270312011-03-01-pojem: <https://slovník.gov.cz/generický/iso-iec-270312011-03-01/pojem/> .
@prefix rdf: <http://www.w3.org/1999/02/22-rdf-syntax-ns#> .
@prefix skos: <http://www.w3.org/2004/02/skos/core#> .
@prefix xsd: <http://www.w3.org/2001/XMLSchema#> .

g-sgov-iso-iec-270312011-03-01:glosář a a-popis-dat-pojem:glosář, skos:ConceptScheme;
  dcterms:title "ISO/IEC 27031:2011-03-01"@cs;
  skos:hasTopConcept g-sgov-iso-iec-270312011-03-01-pojem:cílová-doba-obnovy, g-sgov-iso-iec-270312011-03-01-pojem:kontinuita-podnikání,
    g-sgov-iso-iec-270312011-03-01-pojem:kritický, g-sgov-iso-iec-270312011-03-01-pojem:narušení,
    g-sgov-iso-iec-270312011-03-01-pojem:odolnost, g-sgov-iso-iec-270312011-03-01-pojem:plán-kontinuity-podnikání .

g-sgov-iso-iec-270312011-03-01-pojem:cílová-doba-obnovy a skos:Concept;
  dcterms:source "3.13";
  skos:definition "period of time within which minimum levels of services and/or products and the supporting systems, applications, or functions must be recovered after a disruption has occurred"@en,
    "Časový úsek od havárie, do kterého je nutné obnovit provoz klíčových procesů, neboli představuje maximálně akceptovatelný čas výpadku"@cs;
  skos:inScheme g-sgov-iso-iec-270312011-03-01:glosář;
  skos:prefLabel "Cílová doba obnovy"@cs, "Recovery time objective"@en .

g-sgov-iso-iec-270312011-03-01-pojem:kontinuita-podnikání a skos:Concept;
  dcterms:source "3.2";
  skos:definition "holistic management process that identifies potential threats to an organization and the impacts to business operations whose threats, if realized, might cause, and which provides a framework for building organizational resilience with the capability for an effective response that safeguards the interests of its key stakeholders, reputation, brand and value-creating activities"@en,
    "holistický proces řízení, který identifikuje potenciální hrozby v rámci organizaci a dopadů na obchodní operace, které by hrozby, pokud by mohli nastat, a které poskytují rámec pro budování odolnosti organizace se schopností účinné reakce, která chrání zájmy jejích klíčových zainteresovaných stran "@cs;
  skos:inScheme g-sgov-iso-iec-270312011-03-01:glosář;
  skos:prefLabel "Business Continuity Management"@en, "Kontinuita podnikání "@cs .

g-sgov-iso-iec-270312011-03-01-pojem:kritický a skos:Concept;
  dcterms:source "3.5";
  skos:definition "qualitative description used to emphasize the importance of a resource, process or function that must be available and operational constantly or available and operational at the earliest possible time after an incident, emergency or disaster has occurred"@en;
  skos:inScheme g-sgov-iso-iec-270312011-03-01:glosář;
  skos:prefLabel "Critical"@en, "Kritický"@cs .

g-sgov-iso-iec-270312011-03-01-pojem:narušení a skos:Concept;
  dcterms:source "3.6";
  skos:definition "incident, whether anticipated (e.g. hurricane) or unanticipated (e.g. power failure/outage, earthquake, or attack on ICT systems/infrastructure) which disrupts the normal course of operations at an organization location"@en;
  skos:inScheme g-sgov-iso-iec-270312011-03-01:glosář;
  skos:prefLabel "Disruption"@en, "Narušení"@cs .

g-sgov-iso-iec-270312011-03-01-pojem:odolnost a skos:Concept;
  dcterms:source "3.14";
  skos:definition "ability of an organization to resist being affected by disruptions"@en;
  skos:inScheme g-sgov-iso-iec-270312011-03-01:glosář;
  skos:prefLabel "Odolnost"@cs, "Resilience"@en .

g-sgov-iso-iec-270312011-03-01-pojem:plán-kontinuity-podnikání a skos:Concept;
  dcterms:source "3.3";
  skos:definition """documented procedures that guide organizations to respond, recover, resume, and restore to a pre-defined level of operation following disruption
NOTE　Typically this covers resources, services and activities required to ensure the continuity of critical business functions."""@en,
    "dokumentované postupy, které vedou organizace k tomu, aby při výpadku obnovily předem definovanou úroveň provozu. "@cs;
  skos:inScheme g-sgov-iso-iec-270312011-03-01:glosář;
  skos:prefLabel "Business Continuity Pian"@en, "Plán kontinuity podnikání "@cs .
