@prefix a-popis-dat-pojem: <http://onto.fel.cvut.cz/ontologies/slovník/agendový/popis-dat/pojem/> .
@prefix dcterms: <http://purl.org/dc/terms/> .
@prefix g-sgov-iso-iec-24760-12011-12-15: <https://slovník.gov.cz/generický/iso-iec-24760-12011-12-15/> .
@prefix g-sgov-iso-iec-24760-12011-12-15-pojem: <https://slovník.gov.cz/generický/iso-iec-24760-12011-12-15/pojem/> .
@prefix rdf: <http://www.w3.org/1999/02/22-rdf-syntax-ns#> .
@prefix skos: <http://www.w3.org/2004/02/skos/core#> .
@prefix xsd: <http://www.w3.org/2001/XMLSchema#> .

g-sgov-iso-iec-24760-12011-12-15:glosář a a-popis-dat-pojem:glosář, skos:ConceptScheme;
  dcterms:title "ISO/IEC 24760-1:2011-12-15"@cs;
  skos:hasTopConcept g-sgov-iso-iec-24760-12011-12-15-pojem:evidence-identit, g-sgov-iso-iec-24760-12011-12-15-pojem:federovaná-identita,
    g-sgov-iso-iec-24760-12011-12-15-pojem:identifikace, g-sgov-iso-iec-24760-12011-12-15-pojem:jednotné-přihlášení-identity,
    g-sgov-iso-iec-24760-12011-12-15-pojem:ověření, g-sgov-iso-iec-24760-12011-12-15-pojem:ověření-totožnosti-entity---subjektu,
    g-sgov-iso-iec-24760-12011-12-15-pojem:pseudonym, g-sgov-iso-iec-24760-12011-12-15-pojem:zajištění-identifikace .

g-sgov-iso-iec-24760-12011-12-15-pojem:evidence-identit a skos:Concept;
  dcterms:source "3.4.4";
  skos:definition """identity information (3.2.4) for an entity (3.1.1) required for authentication (3.3.1) of that entity (3.1.1)
NOTE　Identity evidence includes the presented and gathered information related to a claimant that is needed for a successful authentication. Any such information may be part of the authenticated identity for the claimant."""@en;
  skos:inScheme g-sgov-iso-iec-24760-12011-12-15:glosář;
  skos:prefLabel "Evidence identit"@cs, """Identity evidence
evidence of identity"""@en .

g-sgov-iso-iec-24760-12011-12-15-pojem:federovaná-identita a skos:Concept;
  dcterms:source "3.5.1";
  skos:definition """identity (3.1.2) for use in multiple domains (3.2.3), which together form an identity federation (3.5.2)
NOTE 1　A federated identity may be jointly managed by identity information providers of the federated domains.
NOTE 2　The shared attributes used in the federated domains may in particular be used for identification, e.g. to support single-sign-on (SSO).
NOTE 3　The federated identity may persist or may be a temporary one, e.g. as single-sign-on identity."""@en;
  skos:inScheme g-sgov-iso-iec-24760-12011-12-15:glosář;
  skos:prefLabel "Federated Identity"@en, "Federovaná identita"@cs .

g-sgov-iso-iec-24760-12011-12-15-pojem:identifikace a skos:Concept;
  dcterms:source "3.2.1";
  skos:definition """process of recognizing an entity (3.1.1) in a particular domain (3.2.3) as distinct from other entities
NOTE 1　The process of identification applies verification to claimed or observed attributes.
NOTE 2　Identification typically is part of the interactions between an entity and the services in a domain and to access resources. Identification may occur multiple times while the entity is known in the domain."""@en;
  skos:inScheme g-sgov-iso-iec-24760-12011-12-15:glosář;
  skos:prefLabel "Identification"@en, "Identifikace"@cs .

g-sgov-iso-iec-24760-12011-12-15-pojem:jednotné-přihlášení-identity a skos:Concept;
  dcterms:source "3.5.3";
  skos:definition """identity (3.1.2) that includes a single identity assertion (3.3.8) that can be verified (3.2.2) by a relying party (3.3.7) in multiple domains (3.2.3)
NOTE　The identity assertion in a single-sign-on identity is created during authentication of an entity in one domain and can be used in authentication of the entity in any other domain in the same identity federation."""@en,
    "schéma ověřování, které umožňuje uživateli přihlásit se pomocí jediného ID do kteréhokoli z několika souvisejících, ale nezávislých softwarových systémů"@cs;
  skos:inScheme g-sgov-iso-iec-24760-12011-12-15:glosář;
  skos:prefLabel "Jednotné přihlášení identity "@cs, "Single-Sign-On Identity"@en .

g-sgov-iso-iec-24760-12011-12-15-pojem:ověření a skos:Concept;
  dcterms:source "3.2.2";
  skos:definition """process to determine that presented identity information (3.2.4) associated with a particular entity (3.1.1) is applicable for the entity to be recognized in a particular domain (3.2.3) at some point in time
NOTE　Verification can involve checking that the required attributes are present, have the correct syntax, and exist within a defined validity period."""@en;
  skos:inScheme g-sgov-iso-iec-24760-12011-12-15:glosář;
  skos:prefLabel "Ověření"@cs, "Verification"@en .

g-sgov-iso-iec-24760-12011-12-15-pojem:ověření-totožnosti-entity---subjektu a skos:Concept;
  dcterms:source "3.4.2";
  skos:definition """particular form of authentication (3.3.1) based on identity evidence (3.4.4) that is performed as the condition for enrolment (3.4.3)
NOTE 1　Typically identity proofing involves an extensive verification of provided identity information and may include screening, vetting and uniqueness checks, possibly based on biometric techniques.
NOTE 2　Authentication, at the heart of identity proofing, typically is based on an enrolment policy that includes specification of the verification criteria of the identity evidence provided by the entity.
NOTE 3　The authenticated identity that is the result of the authentication in identity proofing may during subsequent enrolment be included in the registration and may serve to facilitate future identification of the entity."""@en;
  skos:inScheme g-sgov-iso-iec-24760-12011-12-15:glosář;
  skos:prefLabel """Identity proofing
initial entity authentication"""@en, "Ověření totožnosti entity / subjektu"@cs .

g-sgov-iso-iec-24760-12011-12-15-pojem:pseudonym a skos:Concept;
  dcterms:source "3.6.3";
  skos:definition """identifier (3.1.4) that contains the minimal identity information (3.2.4) sufficient to allow a verifier (3.3.6) to establish it as a link to a known identity (3.1.2)
NOTE 1　A pseudonym can be used to reduce privacy risks that are associated with the use of identifiers with fixed or known values.
NOTE 2　A pseudonym can be an identifier with a value chosen by the person, or assigned randomly."""@en;
  skos:inScheme g-sgov-iso-iec-24760-12011-12-15:glosář;
  skos:prefLabel "Pseudonym"@cs, "Pseudonym"@en .

g-sgov-iso-iec-24760-12011-12-15-pojem:zajištění-identifikace a skos:Concept;
  dcterms:source "3.3.9";
  skos:definition """level of assurance in the result of identification (3.2.1)
NOTE　Identity assurance expresses the level of confidence in provenance, integrity and applicability of identity information including confidence in identity information maintenance."""@en;
  skos:inScheme g-sgov-iso-iec-24760-12011-12-15:glosář;
  skos:prefLabel "Identity assurance"@en, "Zajištění identifikace"@cs .
