@prefix a-popis-dat-pojem: <http://onto.fel.cvut.cz/ontologies/slovník/agendový/popis-dat/pojem/> .
@prefix dcterms: <http://purl.org/dc/terms/> .
@prefix g-sgov-iso-iec-291152013-04-01: <https://slovník.gov.cz/generický/iso-iec-291152013-04-01/> .
@prefix g-sgov-iso-iec-291152013-04-01-pojem: <https://slovník.gov.cz/generický/iso-iec-291152013-04-01/pojem/> .
@prefix rdf: <http://www.w3.org/1999/02/22-rdf-syntax-ns#> .
@prefix skos: <http://www.w3.org/2004/02/skos/core#> .
@prefix xsd: <http://www.w3.org/2001/XMLSchema#> .

g-sgov-iso-iec-291152013-04-01:glosář a a-popis-dat-pojem:glosář, skos:ConceptScheme;
  dcterms:title "ISO/IEC 29115:2013-04-01"@cs;
  skos:hasTopConcept g-sgov-iso-iec-291152013-04-01-pojem:autentizační-faktor, g-sgov-iso-iec-291152013-04-01-pojem:důvěryhodnost,
    g-sgov-iso-iec-291152013-04-01-pojem:ověřovací-perioda, g-sgov-iso-iec-291152013-04-01-pojem:sdílené-tajemství .

g-sgov-iso-iec-291152013-04-01-pojem:autentizační-faktor a skos:Concept;
  dcterms:source "3.3";
  skos:definition """piece of information and/or process used to authenticate or verify the identity of an entity
[ISO/IEC 19790]
NOTE　Authentication factors are divided into four categories:
- something an entity has (e.g., device signature, passport, hardware device containing a credential, private key);
- something an entity knows (e.g., password, PIN);
- something an entity is (e.g., biometric characteristic); or
- something an entity typically does (e.g., behaviour pattern)."""@en;
  skos:inScheme g-sgov-iso-iec-291152013-04-01:glosář;
  skos:prefLabel "Autentizační faktor"@cs, "authentication factor"@en .

g-sgov-iso-iec-291152013-04-01-pojem:důvěryhodnost a skos:Concept;
  dcterms:source "3.28";
  skos:definition "set of requirements and enforcement mechanisms for parties exchanging identity information"@en;
  skos:inScheme g-sgov-iso-iec-291152013-04-01:glosář;
  skos:prefLabel "Důvěryhodnost"@cs, "Trust Framework"@en .

g-sgov-iso-iec-291152013-04-01-pojem:ověřovací-perioda a skos:Concept;
  dcterms:source "3.30";
  skos:definition "time period during which an identity or credential may be used in one or more transactions"@en;
  skos:inScheme g-sgov-iso-iec-291152013-04-01:glosář;
  skos:prefLabel "Ověřovací perioda"@cs, "Validity Period"@en .

g-sgov-iso-iec-291152013-04-01-pojem:sdílené-tajemství a skos:Concept;
  dcterms:source "3.25";
  skos:definition "secret used in authentication that is known only to the entity and the verifier"@en;
  skos:inScheme g-sgov-iso-iec-291152013-04-01:glosář;
  skos:prefLabel "Sdílené tajemství"@cs, "Shared Secret"@en .
