@prefix a-popis-dat-pojem: <http://onto.fel.cvut.cz/ontologies/slovník/agendový/popis-dat/pojem/> .
@prefix dcterms: <http://purl.org/dc/terms/> .
@prefix g-sgov-iso-iec-270322012-07-15: <https://slovník.gov.cz/generický/iso-iec-270322012-07-15/> .
@prefix g-sgov-iso-iec-270322012-07-15-pojem: <https://slovník.gov.cz/generický/iso-iec-270322012-07-15/pojem/> .
@prefix rdf: <http://www.w3.org/1999/02/22-rdf-syntax-ns#> .
@prefix skos: <http://www.w3.org/2004/02/skos/core#> .
@prefix xsd: <http://www.w3.org/2001/XMLSchema#> .

g-sgov-iso-iec-270322012-07-15:glosář a a-popis-dat-pojem:glosář, skos:ConceptScheme;
  dcterms:title "ISO/IEC 27032:2012-07-15"@cs;
  skos:hasTopConcept g-sgov-iso-iec-270322012-07-15-pojem:aplikační-služba, g-sgov-iso-iec-270322012-07-15-pojem:bot-robot,
    g-sgov-iso-iec-270322012-07-15-pojem:botnet, g-sgov-iso-iec-270322012-07-15-pojem:hacking,
    g-sgov-iso-iec-270322012-07-15-pojem:hactivism, g-sgov-iso-iec-270322012-07-15-pojem:internet,
    g-sgov-iso-iec-270322012-07-15-pojem:internetová-bezpečnost, g-sgov-iso-iec-270322012-07-15-pojem:internetová-kriminalita,
    g-sgov-iso-iec-270322012-07-15-pojem:internetové-služba, g-sgov-iso-iec-270322012-07-15-pojem:kybernetická-bezpečnost,
    g-sgov-iso-iec-270322012-07-15-pojem:kybernetická-kriminalita, g-sgov-iso-iec-270322012-07-15-pojem:poskytovatel-aplikační-služby,
    g-sgov-iso-iec-270322012-07-15-pojem:poskytovatel-internetových-služeb, g-sgov-iso-iec-270322012-07-15-pojem:trojský-kůň,
    g-sgov-iso-iec-270322012-07-15-pojem:vektor-útoku, g-sgov-iso-iec-270322012-07-15-pojem:virtuální-aktiva,
    g-sgov-iso-iec-270322012-07-15-pojem:virtuální-svět, g-sgov-iso-iec-270322012-07-15-pojem:výzvědný-sw .

g-sgov-iso-iec-270322012-07-15-pojem:aplikační-služba a skos:Concept;
  dcterms:source "4.4";
  skos:definition "Software s funkcí poskytovanou na vyžádání předplatitelům prostřednictvím online modelu, který zahrnuje webové aplikace nebo aplikace typu klient-server"@cs,
    "software with functionality delivered on-demand to subscribers through an online model which includes web based or client-server applications"@en;
  skos:inScheme g-sgov-iso-iec-270322012-07-15:glosář;
  skos:prefLabel "Aplikační služba"@cs, "Application Services"@en .

g-sgov-iso-iec-270322012-07-15-pojem:bot-robot a skos:Concept;
  dcterms:source "4.12";
  skos:definition """automated software program used to carry out specific tasks
NOTE 1　The word is often used to describe programs, usually run on a server, that automate tasks such as forwarding or sorting e-mail.
NOTE 2　A bot is also described as a program that operates as an agent for a user or another program or simulates a human activity. On the Internet, the most ubiquitous bots are the programs, also called spiders or crawlers, which access websites and gather their content for search engine indexes."""@en;
  skos:inScheme g-sgov-iso-iec-270322012-07-15:glosář;
  skos:prefLabel "Bot Robot"@en, "Bot robot"@cs .

g-sgov-iso-iec-270322012-07-15-pojem:botnet a skos:Concept;
  dcterms:source "4.13";
  skos:definition "remote control software, specifically a collection of malicious bots, that run autonomously or automatically on compromised computers"@en;
  skos:inScheme g-sgov-iso-iec-270322012-07-15:glosář;
  skos:prefLabel "Botnet"@cs, "Botnet"@en .

g-sgov-iso-iec-270322012-07-15-pojem:hacking a skos:Concept;
  dcterms:source "4.25";
  skos:definition "intentionally accessing a computer system without the authorization of the user or the owner"@en;
  skos:inScheme g-sgov-iso-iec-270322012-07-15:glosář;
  skos:prefLabel "Hacking"@cs, "Hacking"@en .

g-sgov-iso-iec-270322012-07-15-pojem:hactivism a skos:Concept;
  dcterms:source "4.26";
  skos:definition "hacking for a politically or socially motivated purpose"@en;
  skos:inScheme g-sgov-iso-iec-270322012-07-15:glosář;
  skos:prefLabel "Hactivism"@cs, "Hactivism"@en .

g-sgov-iso-iec-270322012-07-15-pojem:internet a skos:Concept;
  dcterms:source "4.29";
  skos:definition """global system of inter-connected networks in the public domain
[ISO/IEC 27033-1:2009]
NOTE　There is a difference between the definition of “an internet” and “the Internet”."""@en;
  skos:inScheme g-sgov-iso-iec-270322012-07-15:glosář;
  skos:prefLabel "Internet"@cs, "The Internet"@en .

g-sgov-iso-iec-270322012-07-15-pojem:internetová-bezpečnost a skos:Concept;
  dcterms:source "4.32";
  skos:definition "preservation of confidentiality, integrity and availability of information in the Internet"@en;
  skos:inScheme g-sgov-iso-iec-270322012-07-15:glosář;
  skos:prefLabel "Internet security"@en, "Internetová bezpečnost "@cs .

g-sgov-iso-iec-270322012-07-15-pojem:internetová-kriminalita a skos:Concept;
  dcterms:source "4.30";
  skos:definition "criminal activity where services or applications in the Internet are used for or are the target of a crime, or where the Internet is the source, tool, target, or place of a crime"@en;
  skos:inScheme g-sgov-iso-iec-270322012-07-15:glosář;
  skos:prefLabel "Internet crime"@en, "Internetová kriminalita"@cs .

g-sgov-iso-iec-270322012-07-15-pojem:internetové-služba a skos:Concept;
  dcterms:source "4.33";
  skos:definition "services delivered to a user to enable access to the Internet via an assigned IP address, which typically include authentication, authorization and domain name services"@en;
  skos:inScheme g-sgov-iso-iec-270322012-07-15:glosář;
  skos:prefLabel "Internet services"@en, "Internetové služba "@cs .

g-sgov-iso-iec-270322012-07-15-pojem:kybernetická-bezpečnost a skos:Concept;
  dcterms:source "4.19", "4.20";
  skos:definition """condition of being protected against physical, social, spiritual, financial, political, emotional, occupational, psychological, educational or other types or consequences of failure, damage, error, accidents, harm or any other event in the Cyberspace which could be considered non-desirable
NOTE 1　This can take the form of being protected from the event or from exposure to something that causes health or economic losses. It can include protection of people or of assets.
NOTE 2　Safety in general is also defined as the state of being certain that adverse effects will not be caused by some agent under defined conditions."""@en,
    """preservation of confidentiality, integrity and availability of information in the Cyberspace
NOTE 1　In addition, other properties, such as authenticity, accountability, non-repudiation, and reliability can also be involved.
NOTE 2　Adapted from the definition for information security in ISO/IEC 27000:2009."""@en;
  skos:inScheme g-sgov-iso-iec-270322012-07-15:glosář;
  skos:prefLabel "Cybersafety"@en, """Cybersecurity
Cyberspace security"""@en, "Kybernetická bezpečnost"@cs .

g-sgov-iso-iec-270322012-07-15-pojem:kybernetická-kriminalita a skos:Concept;
  dcterms:source "4.18";
  skos:definition "criminal activity where services or applications in the Cyberspace are used for or are the target of a crime, or where the Cyberspace is the source, tool, target, or place of a crime"@en;
  skos:inScheme g-sgov-iso-iec-270322012-07-15:glosář;
  skos:prefLabel "Cybercrime"@en, "Kybernetická kriminalita"@cs .

g-sgov-iso-iec-270322012-07-15-pojem:poskytovatel-aplikační-služby a skos:Concept;
  dcterms:source "4.3";
  skos:definition """operator who provides a hosted software solution that provides application services which includes web based or client-server delivery models
EXAMPLE　Online game operators, office application providers and online storage providers."""@en;
  skos:inScheme g-sgov-iso-iec-270322012-07-15:glosář;
  skos:prefLabel "Application Service Provider"@en, "Poskytovatel aplikační služby"@cs .

g-sgov-iso-iec-270322012-07-15-pojem:poskytovatel-internetových-služeb a skos:Concept;
  dcterms:source "4.34";
  skos:definition """organization that provides Internet services to a user and enables its customers access to the Internet
NOTE　Also sometimes referred to as an Internet access provider."""@en;
  skos:inScheme g-sgov-iso-iec-270322012-07-15:glosář;
  skos:prefLabel "Internet service provider"@en, "Poskytovatel internetových služeb"@cs .

g-sgov-iso-iec-270322012-07-15-pojem:trojský-kůň a skos:Concept;
  dcterms:source "4.47";
  skos:definition "malware that appears to perform a desirable function"@en;
  skos:inScheme g-sgov-iso-iec-270322012-07-15:glosář;
  skos:prefLabel "Trojan Horse"@en, "Trojský kůň"@cs .

g-sgov-iso-iec-270322012-07-15-pojem:vektor-útoku a skos:Concept;
  dcterms:source "4.10";
  skos:definition "path or means by which an attacker can gain access to a computer or network server in order to deliver a malicious outcome"@en;
  skos:inScheme g-sgov-iso-iec-270322012-07-15:glosář;
  skos:prefLabel "Attack Vector"@en, "Vektor útoku"@cs .

g-sgov-iso-iec-270322012-07-15-pojem:virtuální-aktiva a skos:Concept;
  dcterms:source "4.49";
  skos:definition """representation of an asset in the Cyberspace
NOTE　In this context, currency can be defined as either a medium of exchange or a property that has value in a specific environment, such as a video game or a financial trading simulation exercise."""@en;
  skos:inScheme g-sgov-iso-iec-270322012-07-15:glosář;
  skos:prefLabel "Virtual Asset"@en, "Virtuální aktiva"@cs .

g-sgov-iso-iec-270322012-07-15-pojem:virtuální-svět a skos:Concept;
  dcterms:source "4.51";
  skos:definition """simulated environment accessed by multiple users through an online interface
NOTE 1　The simulated environments are often interactive.
NOTE 2　The physical world in which people live, and the related characteristics, will be referred to as the “real world” to differentiate it from a virtual world."""@en;
  skos:inScheme g-sgov-iso-iec-270322012-07-15:glosář;
  skos:prefLabel "Virtual World"@en, "Virtuální svět"@cs .

g-sgov-iso-iec-270322012-07-15-pojem:výzvědný-sw a skos:Concept;
  dcterms:source "4.43";
  skos:definition """deceptive software that collects private or confidential information from a computer user
NOTE　Information can include matters such as websites most frequently visited or more sensitive information such as passwords."""@en;
  skos:inScheme g-sgov-iso-iec-270322012-07-15:glosář;
  skos:prefLabel "Spyware"@en, "Výzvědný SW"@cs .
