@prefix a-popis-dat-pojem: <http://onto.fel.cvut.cz/ontologies/slovník/agendový/popis-dat/pojem/> .
@prefix dcterms: <http://purl.org/dc/terms/> .
@prefix g-sgov-iso-iec-197902012-08-15: <https://slovník.gov.cz/generický/iso-iec-197902012-08-15/> .
@prefix g-sgov-iso-iec-197902012-08-15-pojem: <https://slovník.gov.cz/generický/iso-iec-197902012-08-15/pojem/> .
@prefix rdf: <http://www.w3.org/1999/02/22-rdf-syntax-ns#> .
@prefix skos: <http://www.w3.org/2004/02/skos/core#> .
@prefix xsd: <http://www.w3.org/2001/XMLSchema#> .

g-sgov-iso-iec-197902012-08-15:glosář a a-popis-dat-pojem:glosář, skos:ConceptScheme;
  dcterms:title "ISO/IEC 19790:2012-08-15"@cs;
  skos:hasTopConcept g-sgov-iso-iec-197902012-08-15-pojem:citlivá-data, g-sgov-iso-iec-197902012-08-15-pojem:entita,
    g-sgov-iso-iec-197902012-08-15-pojem:heslo, g-sgov-iso-iec-197902012-08-15-pojem:klíč-soukromý,
    g-sgov-iso-iec-197902012-08-15-pojem:kódovací-klíč, g-sgov-iso-iec-197902012-08-15-pojem:osobní-identifikační-kód,
    g-sgov-iso-iec-197902012-08-15-pojem:provozní-prostředí, g-sgov-iso-iec-197902012-08-15-pojem:role,
    g-sgov-iso-iec-197902012-08-15-pojem:seznam-přístupů, g-sgov-iso-iec-197902012-08-15-pojem:tajný-klíč,
    g-sgov-iso-iec-197902012-08-15-pojem:veřejný-klíč, g-sgov-iso-iec-197902012-08-15-pojem:řízení-přístupu-založené-na-rolích .

g-sgov-iso-iec-197902012-08-15-pojem:citlivá-data a skos:Concept;
  dcterms:source "3.109";
  skos:definition "data that, in user’s view, requires protection"@en;
  skos:inScheme g-sgov-iso-iec-197902012-08-15:glosář;
  skos:prefLabel "Citlivá data"@cs, "Sensitive Data"@en .

g-sgov-iso-iec-197902012-08-15-pojem:entita a skos:Concept;
  dcterms:source "3.37";
  skos:definition "person, group, device or process"@en;
  skos:inScheme g-sgov-iso-iec-197902012-08-15:glosář;
  skos:prefLabel "Entita"@cs, "Entity"@en .

g-sgov-iso-iec-197902012-08-15-pojem:heslo a skos:Concept;
  dcterms:source "3.88";
  skos:definition """string of characters used to authenticate an identity or to verify access authorisation
EXAMPLE　Letters, numbers, and other symbols."""@en;
  skos:inScheme g-sgov-iso-iec-197902012-08-15:glosář;
  skos:prefLabel "Heslo"@cs, "Password"@en .

g-sgov-iso-iec-197902012-08-15-pojem:klíč-soukromý a skos:Concept;
  dcterms:source "3.94";
  skos:definition """key of an entity's asymmetric key pair, which should only be used by that entity
NOTE　In the case of an asymmetric signature system the private key defines the signature transformation. In the case of an asymmetric encipherment system the private key defines the decipherment transformation."""@en;
  skos:inScheme g-sgov-iso-iec-197902012-08-15:glosář;
  skos:prefLabel "Klíč soukromý"@cs, "Private Key"@en .

g-sgov-iso-iec-197902012-08-15-pojem:kódovací-klíč a skos:Concept;
  dcterms:source "3.36";
  skos:definition """cryptographic key that has been encrypted using an approved security function with a key encryption key
NOTE　It is considered protected."""@en;
  skos:inScheme g-sgov-iso-iec-197902012-08-15:glosář;
  skos:prefLabel "Kódovací klíč"@cs, "encrypted key"@en .

g-sgov-iso-iec-197902012-08-15-pojem:osobní-identifikační-kód a skos:Concept;
  dcterms:source "3.89";
  skos:definition "numeric code used to authenticate an identity"@en;
  skos:inScheme g-sgov-iso-iec-197902012-08-15:glosář;
  skos:prefLabel "Osobní identifikační kód"@cs, "Personal Identification Number"@en .

g-sgov-iso-iec-197902012-08-15-pojem:provozní-prostředí a skos:Concept;
  dcterms:source "3.83";
  skos:definition "set of all software and hardware consisting of an operating system and hardware platform required for the module to operate securely"@en;
  skos:inScheme g-sgov-iso-iec-197902012-08-15:glosář;
  skos:prefLabel "Operational environment"@en, "Provozní prostředí"@cs .

g-sgov-iso-iec-197902012-08-15-pojem:role a skos:Concept;
  dcterms:source "3.102";
  skos:definition """security attribute associated to a user defining the user access rights or limitations to services of a cryptographic module
NOTE　One or more services can be associated to a role. A role can be associated to one or more users and a user can assume one or more roles."""@en;
  skos:inScheme g-sgov-iso-iec-197902012-08-15:glosář;
  skos:prefLabel "Role"@cs, "Role"@en .

g-sgov-iso-iec-197902012-08-15-pojem:seznam-přístupů a skos:Concept;
  dcterms:source "3.1";
  skos:definition "list of permissions to grant access to an object"@en;
  skos:inScheme g-sgov-iso-iec-197902012-08-15:glosář;
  skos:prefLabel "Access control list"@en, "Seznam přístupů"@cs .

g-sgov-iso-iec-197902012-08-15-pojem:tajný-klíč a skos:Concept;
  dcterms:source "3.105";
  skos:definition "cryptographic key, used with a secret key cryptographic algorithm that is uniquely associated with one or more entities and should not be made public"@en;
  skos:inScheme g-sgov-iso-iec-197902012-08-15:glosář;
  skos:prefLabel "Secret Key"@en, "Tajný klíč"@cs .

g-sgov-iso-iec-197902012-08-15-pojem:veřejný-klíč a skos:Concept;
  dcterms:source "3.96";
  skos:definition """key of an entity's asymmetric key pair, which can be made public
NOTE 1　In the case of an asymmetric signature system the public key defines the verification transformation. In the case of an asymmetric encipherment system the public key defines the encipherment transformation. A key that is 'publicly known' is not necessarily globally available. The key can only be available to all members of a pre-specified group.
NOTE 2　For the purposes of this International Standard, public keys are not considered CSPs."""@en;
  skos:inScheme g-sgov-iso-iec-197902012-08-15:glosář;
  skos:prefLabel "Public Key"@en, "Veřejný klíč"@cs .

g-sgov-iso-iec-197902012-08-15-pojem:řízení-přístupu-založené-na-rolích a skos:Concept;
  dcterms:source "3.103";
  skos:definition "permissions attributed to a role granting access to an object"@en;
  skos:inScheme g-sgov-iso-iec-197902012-08-15:glosář;
  skos:prefLabel "Role-Based Access Control"@en, "Řízení přístupu založené na rolích"@cs .
