@prefix a-popis-dat-pojem: <http://onto.fel.cvut.cz/ontologies/slovník/agendový/popis-dat/pojem/> .
@prefix dcterms: <http://purl.org/dc/terms/> .
@prefix g-sgov-iso-iec-291002011-12-15: <https://slovník.gov.cz/generický/iso-iec-291002011-12-15/> .
@prefix g-sgov-iso-iec-291002011-12-15-pojem: <https://slovník.gov.cz/generický/iso-iec-291002011-12-15/pojem/> .
@prefix rdf: <http://www.w3.org/1999/02/22-rdf-syntax-ns#> .
@prefix skos: <http://www.w3.org/2004/02/skos/core#> .
@prefix xsd: <http://www.w3.org/2001/XMLSchema#> .

g-sgov-iso-iec-291002011-12-15:glosář a a-popis-dat-pojem:glosář, skos:ConceptScheme;
  dcterms:title "ISO/IEC 29100:2011-12-15"@cs;
  skos:hasTopConcept g-sgov-iso-iec-291002011-12-15-pojem:anonymita, g-sgov-iso-iec-291002011-12-15-pojem:anonymizace,
    g-sgov-iso-iec-291002011-12-15-pojem:anonymizovaná-data, g-sgov-iso-iec-291002011-12-15-pojem:identita-osoby,
    g-sgov-iso-iec-291002011-12-15-pojem:politika-soukromí, g-sgov-iso-iec-291002011-12-15-pojem:porušení-soukromí,
    g-sgov-iso-iec-291002011-12-15-pojem:pseudonymizace, g-sgov-iso-iec-291002011-12-15-pojem:třetí-strana,
    g-sgov-iso-iec-291002011-12-15-pojem:řízení-soukromí .

g-sgov-iso-iec-291002011-12-15-pojem:identita-osoby a skos:Concept;
  dcterms:source "2021-07-02 00:00:00";
  skos:definition "Identita je sada vlastností, které jednoznačně určují konkrétní osobu."@cs;
  skos:inScheme g-sgov-iso-iec-291002011-12-15:glosář;
  skos:prefLabel "Identita (osoby)"@cs;
  skos:scopeNote "Identita souvisí s bytím a není to jenom jméno, a už vůbec ne role."@cs .

g-sgov-iso-iec-291002011-12-15-pojem:anonymita a skos:Concept;
  dcterms:source "2.1";
  skos:definition "characteristic of information that does not permit a personally identifiable information principal to be identified directly or indirectly"@en;
  skos:inScheme g-sgov-iso-iec-291002011-12-15:glosář;
  skos:prefLabel "Anonymita"@cs, "Anonymity"@en .

g-sgov-iso-iec-291002011-12-15-pojem:anonymizace a skos:Concept;
  dcterms:source "2.2";
  skos:definition "process by which personally identifiable information (PII) is irreversibly altered in such a way that a PII principal can no longer be identified directly or indirectly, either by the PII controller alone or in collaboration with any other party"@en;
  skos:inScheme g-sgov-iso-iec-291002011-12-15:glosář;
  skos:prefLabel "Anonymizace"@cs, "Anonymization"@en .

g-sgov-iso-iec-291002011-12-15-pojem:anonymizovaná-data a skos:Concept;
  dcterms:source "2.3";
  skos:definition "data that has been produced as the output of a personally identifiable information anonymization process"@en;
  skos:inScheme g-sgov-iso-iec-291002011-12-15:glosář;
  skos:prefLabel "Anonymized data"@en, "Anonymizovaná data"@cs .

g-sgov-iso-iec-291002011-12-15-pojem:politika-soukromí a skos:Concept;
  dcterms:source "2.16";
  skos:definition "overall intention and direction, rules and commitment, as formally expressed by the personally identifiable information (PII) controller related to the processing of PII in a particular setting"@en;
  skos:inScheme g-sgov-iso-iec-291002011-12-15:glosář;
  skos:prefLabel "Politika soukromí"@cs, "Privacy Policy"@en .

g-sgov-iso-iec-291002011-12-15-pojem:porušení-soukromí a skos:Concept;
  dcterms:source "2.13";
  skos:definition "situation where personally identifiable information is processed in violation of one or more relevant privacy safeguarding requirements"@en;
  skos:inScheme g-sgov-iso-iec-291002011-12-15:glosář;
  skos:prefLabel "Porušení soukromí"@cs, "Privacy Breach"@en .

g-sgov-iso-iec-291002011-12-15-pojem:pseudonymizace a skos:Concept;
  dcterms:source "2.24";
  skos:definition """process applied to personally identifiable information (PII) which replaces identifying information with an alias
NOTE 1　Pseudonymization can be performed either by PII principals themselves or by PII controllers. Pseudonymization can be used by PII principals to consistently use a resource or service without disclosing their identity to this resource or service (or between services), while still being held accountable for that use.
NOTE 2　Pseudonymization does not rule out the possibility that there might be (a restricted set of) privacy stakeholders other than the PII controller of the pseudonymized data which are able to determine the PII principal’s identity based on the alias and data linked to it."""@en;
  skos:inScheme g-sgov-iso-iec-291002011-12-15:glosář;
  skos:prefLabel "Pseudonymizace"@cs, "Pseudonymization"@en .

g-sgov-iso-iec-291002011-12-15-pojem:třetí-strana a skos:Concept;
  dcterms:source "2.27";
  skos:definition "privacy stakeholder other than the personally identifiable information (PII) principal, the PII controller and the PII processor, and the natural persons who are authorized to process the data under the direct authority of the PII controller or the PII processor"@en;
  skos:inScheme g-sgov-iso-iec-291002011-12-15:glosář;
  skos:prefLabel "Third Party"@en, "Třetí strana"@cs .

g-sgov-iso-iec-291002011-12-15-pojem:řízení-soukromí a skos:Concept;
  dcterms:source "2.14";
  skos:definition """measures that treat privacy risks by reducing their likelihood or their consequences
NOTE 1　Privacy controls include organizational, physical and technical measures, e.g., policies, procedures, guidelines, legal contracts, management practices or organizational structures.
NOTE 2　Control is also used as a synonym for safeguard or countermeasure."""@en;
  skos:inScheme g-sgov-iso-iec-291002011-12-15:glosář;
  skos:prefLabel "Privacy Controls"@en, "Řízení soukromí"@cs .
