@prefix a-popis-dat-pojem: <http://onto.fel.cvut.cz/ontologies/slovník/agendový/popis-dat/pojem/> .
@prefix dcterms: <http://purl.org/dc/terms/> .
@prefix g-sgov-iso-iec-27033-12015-08-15: <https://slovník.gov.cz/generický/iso-iec-27033-12015-08-15/> .
@prefix g-sgov-iso-iec-27033-12015-08-15-pojem: <https://slovník.gov.cz/generický/iso-iec-27033-12015-08-15/pojem/> .
@prefix rdf: <http://www.w3.org/1999/02/22-rdf-syntax-ns#> .
@prefix skos: <http://www.w3.org/2004/02/skos/core#> .
@prefix xsd: <http://www.w3.org/2001/XMLSchema#> .

g-sgov-iso-iec-27033-12015-08-15:glosář a a-popis-dat-pojem:glosář, skos:ConceptScheme;
  dcterms:title "ISO/IEC 27033-1:2015-08-15"@cs;
  skos:hasTopConcept g-sgov-iso-iec-27033-12015-08-15-pojem:administrace-sítě, g-sgov-iso-iec-27033-12015-08-15-pojem:analyzátor-sítě,
    g-sgov-iso-iec-27033-12015-08-15-pojem:demilitarizovaná-zóna, g-sgov-iso-iec-27033-12015-08-15-pojem:extranet,
    g-sgov-iso-iec-27033-12015-08-15-pojem:filtrování, g-sgov-iso-iec-27033-12015-08-15-pojem:firewall,
    g-sgov-iso-iec-27033-12015-08-15-pojem:internet, g-sgov-iso-iec-27033-12015-08-15-pojem:intranet,
    g-sgov-iso-iec-27033-12015-08-15-pojem:politika-bezpečnosti-sítě, g-sgov-iso-iec-27033-12015-08-15-pojem:port-zásuvka,
    g-sgov-iso-iec-27033-12015-08-15-pojem:prevence-vniknutí, g-sgov-iso-iec-27033-12015-08-15-pojem:přepínač,
    g-sgov-iso-iec-27033-12015-08-15-pojem:směrovač, g-sgov-iso-iec-27033-12015-08-15-pojem:síťový-čmuchač,
    g-sgov-iso-iec-27033-12015-08-15-pojem:tunel, g-sgov-iso-iec-27033-12015-08-15-pojem:upozornění,
    g-sgov-iso-iec-27033-12015-08-15-pojem:vniknutí, g-sgov-iso-iec-27033-12015-08-15-pojem:vzdálený-přístup,
    g-sgov-iso-iec-27033-12015-08-15-pojem:vzdálený-uživatel, g-sgov-iso-iec-27033-12015-08-15-pojem:útočník,
    g-sgov-iso-iec-27033-12015-08-15-pojem:řízení-sítě .

g-sgov-iso-iec-27033-12015-08-15-pojem:administrace-sítě a skos:Concept;
  dcterms:source "3.24";
  skos:definition "day-to-day operation and management of network processes, and assets using networks"@en;
  skos:inScheme g-sgov-iso-iec-27033-12015-08-15:glosář;
  skos:prefLabel "Administrace sítě"@cs, "Network Administration"@en .

g-sgov-iso-iec-27033-12015-08-15-pojem:analyzátor-sítě a skos:Concept;
  dcterms:source "3.25";
  skos:definition """device or software used to observe and analyse information flowing in networks
Note 1 to entry: Prior to the information flow analysis, information should be gathered in a specific way such as by using a network sniffer."""@en;
  skos:inScheme g-sgov-iso-iec-27033-12015-08-15:glosář;
  skos:prefLabel "Analyzátor sítě"@cs, "Network Analyzer"@en .

g-sgov-iso-iec-27033-12015-08-15-pojem:demilitarizovaná-zóna a skos:Concept;
  dcterms:source "3.8";
  skos:definition "perimeter network (also known as a screened sub-net) inserted as a “neutral zone” between networks"@en;
  skos:inScheme g-sgov-iso-iec-27033-12015-08-15:glosář;
  skos:prefLabel "Demilitarized Zone"@en, "Demilitarizovaná zóna"@cs .

g-sgov-iso-iec-27033-12015-08-15-pojem:extranet a skos:Concept;
  dcterms:source "3.10";
  skos:definition """extension of an organization's Intranet, especially over the public network infrastructure, enabling resource sharing between the organization and other organizations and individuals that it deals with by providing limited access to its Intranet
Note 1 to entry: For example, an organization's customers can be provided access to some part of its Intranet, creating an extranet, but the customers cannot be considered “trusted” from a security standpoint."""@en;
  skos:inScheme g-sgov-iso-iec-27033-12015-08-15:glosář;
  skos:prefLabel "Extranet"@cs, "Extranet"@en .

g-sgov-iso-iec-27033-12015-08-15-pojem:filtrování a skos:Concept;
  dcterms:source "3.11";
  skos:definition "process of accepting or rejecting data flows through a network, according to specified criteria"@en;
  skos:inScheme g-sgov-iso-iec-27033-12015-08-15:glosář;
  skos:prefLabel "Filtering"@en, "Filtrování"@cs .

g-sgov-iso-iec-27033-12015-08-15-pojem:firewall a skos:Concept;
  dcterms:source "3.12";
  skos:definition "type of security barrier placed between network environments — consisting of a dedicated device or a composite of several components and techniques — through which all traffic from one network environment traverses to another, and vice versa, and only authorized traffic, as defined by the local security policy, is allowed to pass"@en;
  skos:inScheme g-sgov-iso-iec-27033-12015-08-15:glosář;
  skos:prefLabel "Firewall"@cs, "firewall"@en .

g-sgov-iso-iec-27033-12015-08-15-pojem:internet a skos:Concept;
  dcterms:source "3.15";
  skos:definition "collection of interconnected networks called an internetwork or just an internet"@en;
  skos:inScheme g-sgov-iso-iec-27033-12015-08-15:glosář;
  skos:prefLabel "Internet"@cs, "Internet"@en .

g-sgov-iso-iec-27033-12015-08-15-pojem:intranet a skos:Concept;
  dcterms:source "3.16";
  skos:definition "private computer network that uses Internet protocols and network connectivity to securely share part of an organization's information or operations with its employees"@en;
  skos:inScheme g-sgov-iso-iec-27033-12015-08-15:glosář;
  skos:prefLabel "Intranet"@cs, "Intranet"@en .

g-sgov-iso-iec-27033-12015-08-15-pojem:politika-bezpečnosti-sítě a skos:Concept;
  dcterms:source "3.29";
  skos:definition "set of statements, rules and practices that explain an organization’s approach to the use of its network resources, and specify how its network infrastructure and services should be protected"@en;
  skos:inScheme g-sgov-iso-iec-27033-12015-08-15:glosář;
  skos:prefLabel "Network Security Policy"@en, "Politika bezpečnosti sítě"@cs .

g-sgov-iso-iec-27033-12015-08-15-pojem:port-zásuvka a skos:Concept;
  dcterms:source "3.31";
  skos:definition """endpoint to a connection
Note 1 to entry: In the context of the Internet protocol, a port is a logical channel endpoint of a TCP connection or UDP messages. Application protocols which are based on TCP or UDP have typically assigned default port numbers, e.g. port 80 for HTTP."""@en;
  skos:inScheme g-sgov-iso-iec-27033-12015-08-15:glosář;
  skos:prefLabel "Port"@en, "Port (zásuvka)"@cs .

g-sgov-iso-iec-27033-12015-08-15-pojem:prevence-vniknutí a skos:Concept;
  dcterms:source "3.20";
  skos:definition "formal process of actively responding to prevent intrusions"@en;
  skos:inScheme g-sgov-iso-iec-27033-12015-08-15:glosář;
  skos:prefLabel "Intrusion prevention"@en, "Prevence vniknutí"@cs .

g-sgov-iso-iec-27033-12015-08-15-pojem:přepínač a skos:Concept;
  dcterms:source "3.39";
  skos:definition "device which provides connectivity between networked devices by means of internal switching mechanisms, with the switching technology typically implemented at layer 2 or layer 3 of the OSI reference model"@en;
  skos:inScheme g-sgov-iso-iec-27033-12015-08-15:glosář;
  skos:prefLabel "Přepínač"@cs, "Switch"@en .

g-sgov-iso-iec-27033-12015-08-15-pojem:směrovač a skos:Concept;
  dcterms:source "3.34";
  skos:definition """network device that is used to establish and control the flow of data between different networks by selecting paths or routes based upon routing protocol mechanisms and algorithms
Note 1 to entry: The networks can themselves be based on different protocols.
Note 2 to entry: The routing information is kept in a routing table."""@en;
  skos:inScheme g-sgov-iso-iec-27033-12015-08-15:glosář;
  skos:prefLabel "Router"@en, "Směrovač"@cs .

g-sgov-iso-iec-27033-12015-08-15-pojem:síťový-čmuchač a skos:Concept;
  dcterms:source "3.30";
  skos:definition "device or software used to capture information flowing in networks"@en;
  skos:inScheme g-sgov-iso-iec-27033-12015-08-15:glosář;
  skos:prefLabel "Network Sniffer"@en, "Síťový čmuchač "@cs .

g-sgov-iso-iec-27033-12015-08-15-pojem:tunel a skos:Concept;
  dcterms:source "3.40";
  skos:definition """data path between networked devices which is established across an existing network infrastructure
Note 1 to entry: Tunnels can be established using techniques such as protocol encapsulation, label switching, or virtual circuits."""@en;
  skos:inScheme g-sgov-iso-iec-27033-12015-08-15:glosář;
  skos:prefLabel "Tunel"@cs, "Tunnel"@en .

g-sgov-iso-iec-27033-12015-08-15-pojem:upozornění a skos:Concept;
  dcterms:source "3.1";
  skos:definition "“instant” indication that an information system and network may be under attack, or in danger because of accident, failure or human error"@en;
  skos:inScheme g-sgov-iso-iec-27033-12015-08-15:glosář;
  skos:prefLabel "Alert"@en, "Upozornění"@cs .

g-sgov-iso-iec-27033-12015-08-15-pojem:vniknutí a skos:Concept;
  dcterms:source "3.17";
  skos:definition "unauthorized access to a network or a network-connected system, i.e. deliberate or accidental unauthorized access to an information system, to include malicious activity against an information system, or unauthorized use of resources within an information system"@en;
  skos:inScheme g-sgov-iso-iec-27033-12015-08-15:glosář;
  skos:prefLabel "Intrusion"@en, "Vniknutí"@cs .

g-sgov-iso-iec-27033-12015-08-15-pojem:vzdálený-přístup a skos:Concept;
  dcterms:source "3.32";
  skos:definition "process of accessing network resources from another network, or from a terminal device which is not permanently connected, physically or logically, to the network it is accessing"@en;
  skos:inScheme g-sgov-iso-iec-27033-12015-08-15:glosář;
  skos:prefLabel "Remote Access"@en, "Vzdálený přístup"@cs .

g-sgov-iso-iec-27033-12015-08-15-pojem:vzdálený-uživatel a skos:Concept;
  dcterms:source "3.33";
  skos:definition "user at a site other than the one at which the network resources being used are located"@en;
  skos:inScheme g-sgov-iso-iec-27033-12015-08-15:glosář;
  skos:prefLabel "Remote User"@en, "Vzdálený uživatel"@cs .

g-sgov-iso-iec-27033-12015-08-15-pojem:útočník a skos:Concept;
  dcterms:source "3.3";
  skos:definition "person deliberately exploiting vulnerabilities in technical and non-technical security controls in order to steal or compromise information systems and networks, or to compromise availability to legitimate users of information system and network resources"@en;
  skos:inScheme g-sgov-iso-iec-27033-12015-08-15:glosář;
  skos:prefLabel "Attacker"@en, "Útočník"@cs .

g-sgov-iso-iec-27033-12015-08-15-pojem:řízení-sítě a skos:Concept;
  dcterms:source "3.27";
  skos:definition "process of planning, designing, implementing, operating, monitoring and maintaining a network"@en;
  skos:inScheme g-sgov-iso-iec-27033-12015-08-15:glosář;
  skos:prefLabel "Network Management"@en, "Řízení sítě"@cs .
