@prefix a-popis-dat-pojem: <http://onto.fel.cvut.cz/ontologies/slovník/agendový/popis-dat/pojem/> .
@prefix dcterms: <http://purl.org/dc/terms/> .
@prefix g-sgov-european-interoperability-reference-architecture: <https://slovník.gov.cz/generický/european-interoperability-reference-architecture/> .
@prefix g-sgov-european-interoperability-reference-architecture-pojem: <https://slovník.gov.cz/generický/european-interoperability-reference-architecture/pojem/> .
@prefix rdf: <http://www.w3.org/1999/02/22-rdf-syntax-ns#> .
@prefix skos: <http://www.w3.org/2004/02/skos/core#> .

g-sgov-european-interoperability-reference-architecture:glosář a a-popis-dat-pojem:glosář,
    skos:ConceptScheme;
  dcterms:title "European interoperability reference architecture"@cs;
  skos:hasTopConcept g-sgov-european-interoperability-reference-architecture-pojem:aplikační-služba,
    g-sgov-european-interoperability-reference-architecture-pojem:cyklus-tvorby-politiky,
    g-sgov-european-interoperability-reference-architecture-pojem:data-údaj, g-sgov-european-interoperability-reference-architecture-pojem:datová-politika,
    g-sgov-european-interoperability-reference-architecture-pojem:datový-model, g-sgov-european-interoperability-reference-architecture-pojem:datový-standard,
    g-sgov-european-interoperability-reference-architecture-pojem:dohoda-o-interoperabilitě,
    g-sgov-european-interoperability-reference-architecture-pojem:evropské-interoperabilní-řešení,
    g-sgov-european-interoperability-reference-architecture-pojem:informace, g-sgov-european-interoperability-reference-architecture-pojem:infrastruktura-digitálních-služeb,
    g-sgov-european-interoperability-reference-architecture-pojem:kalatog-datových-sad,
    g-sgov-european-interoperability-reference-architecture-pojem:katalog-datových-standardů,
    g-sgov-european-interoperability-reference-architecture-pojem:katalog-legislativy,
    g-sgov-european-interoperability-reference-architecture-pojem:katalog-veřejných-služeb,
    g-sgov-european-interoperability-reference-architecture-pojem:m2m-rozhraní, g-sgov-european-interoperability-reference-architecture-pojem:model-dodávky-služeb,
    g-sgov-european-interoperability-reference-architecture-pojem:nástroj-formulace-a-zavedení-politiky,
    g-sgov-european-interoperability-reference-architecture-pojem:občan, g-sgov-european-interoperability-reference-architecture-pojem:organizační-předpoklad-interoperability,
    g-sgov-european-interoperability-reference-architecture-pojem:podpůrné-hledisko-specifikace-interoperability,
    g-sgov-european-interoperability-reference-architecture-pojem:poskytovatel-veřejné-služby,
    g-sgov-european-interoperability-reference-architecture-pojem:prostředek---reprezentace,
    g-sgov-european-interoperability-reference-architecture-pojem:předpoklad-rozvoje-politiky,
    g-sgov-european-interoperability-reference-architecture-pojem:schopnost, g-sgov-european-interoperability-reference-architecture-pojem:služba-choreografie-služeb,
    g-sgov-european-interoperability-reference-architecture-pojem:služba-orchestrace-služeb,
    g-sgov-european-interoperability-reference-architecture-pojem:služby-infrastruktury-pro-hosting-a-síťovou-komunikaci,
    g-sgov-european-interoperability-reference-architecture-pojem:specifikace-byznys-interoperability,
    g-sgov-european-interoperability-reference-architecture-pojem:specifikace-právní-interoperability,
    g-sgov-european-interoperability-reference-architecture-pojem:specifikace-sémantické-interoperability,
    g-sgov-european-interoperability-reference-architecture-pojem:specifikace-technologické-interoperability,
    g-sgov-european-interoperability-reference-architecture-pojem:spotřebitel-veřejné-služby,
    g-sgov-european-interoperability-reference-architecture-pojem:uživatelské-rozhraní,
    g-sgov-european-interoperability-reference-architecture-pojem:veřejná-politika, g-sgov-european-interoperability-reference-architecture-pojem:veřejná-služba,
    g-sgov-european-interoperability-reference-architecture-pojem:výměna-informací, g-sgov-european-interoperability-reference-architecture-pojem:zprostředkovatel-dodávky-veřejné-služby .

g-sgov-european-interoperability-reference-architecture-pojem:aplikační-služba a skos:Concept;
  skos:definition "is an externally visible unit of functionality, provided by one or more application components. It is exposed through well-defined interfaces and is meaningful to the environment. An Application Service exposes the functionality of components to their environment. This functionality is accessed through one or more application interfaces."@en,
    "je externě viditelná jednotka funkčnosti, kterou poskytuje jedna nebo více komponent aplikace. Je vystavena prostřednictvím dobře definovaných rozhraní a je smysluplná pro životní prostředí. Aplikační služba vystavuje funkčnost komponent jejich prostředí. Tato funkce je přístupná prostřednictvím jednoho nebo více aplikačních rozhraní"@cs;
  skos:inScheme g-sgov-european-interoperability-reference-architecture:glosář;
  skos:prefLabel "Aplikační služba"@cs, "Application Service"@en .

g-sgov-european-interoperability-reference-architecture-pojem:cyklus-tvorby-politiky
  a skos:Concept;
  skos:inScheme g-sgov-european-interoperability-reference-architecture:glosář;
  skos:prefLabel "Cyklus tvorby politiky"@cs, "Public Policy Cycle"@en .

g-sgov-european-interoperability-reference-architecture-pojem:data-údaj a skos:Concept;
  skos:definition "is facts represented as text, numbers, graphics, images, sound, or video. Data is the raw material used to represent information, or from which information can be derived."@en;
  skos:inScheme g-sgov-european-interoperability-reference-architecture:glosář;
  skos:prefLabel "Data"@en, "Data (Údaj)"@cs .

g-sgov-european-interoperability-reference-architecture-pojem:datová-politika a skos:Concept;
  skos:inScheme g-sgov-european-interoperability-reference-architecture:glosář;
  skos:prefLabel "Data Policy"@en, "Datová politika"@cs .

g-sgov-european-interoperability-reference-architecture-pojem:datový-model a skos:Concept;
  skos:definition "A data model organizes data elements and standardizes how the data elements relate to one another. Since data elements document real life people, places and things and the events between them, the data model represents reality, for example a house has many windows or a cat has two eyes. Computers are used for the accounting of these real life things and events and therefore the data model is a necessary standard to ensure exact communication between human beings. – Wikipedia"@en;
  skos:inScheme g-sgov-european-interoperability-reference-architecture:glosář;
  skos:prefLabel "Data Model"@en, "Datový model"@cs .

g-sgov-european-interoperability-reference-architecture-pojem:datový-standard a skos:Concept;
  skos:inScheme g-sgov-european-interoperability-reference-architecture:glosář;
  skos:prefLabel "Data Standard"@en, "Datový standard"@cs .

g-sgov-european-interoperability-reference-architecture-pojem:dohoda-o-interoperabilitě
  a skos:Concept;
  skos:inScheme g-sgov-european-interoperability-reference-architecture:glosář;
  skos:prefLabel "Dohoda o interoperabilitě"@cs, "Interoperability Agreement"@en .

g-sgov-european-interoperability-reference-architecture-pojem:evropské-interoperabilní-řešení
  a skos:Concept;
  skos:definition "(IES) is a solution, developed by Public Administrations that facilitate the delivery of electronic Public Services and cross-border exchange of information between Public Administrations (or Citizens) in support to the implementation and advancement of EU, national or local Public Policies."@en;
  skos:inScheme g-sgov-european-interoperability-reference-architecture:glosář;
  skos:prefLabel "Evropské interoperabilní řešení"@cs, "Interoperable European Solution"@en .

g-sgov-european-interoperability-reference-architecture-pojem:informace a skos:Concept;
  skos:definition "is a piece of business data or a group of pieces of business data with a unique business semantics definition in a specific business context [ISO15000-5, UN/CEFACT CCTS]."@en;
  skos:inScheme g-sgov-european-interoperability-reference-architecture:glosář;
  skos:prefLabel "Business Information"@en, "Informace"@cs .

g-sgov-european-interoperability-reference-architecture-pojem:infrastruktura-digitálních-služeb
  a skos:Concept;
  skos:definition "Jedná se o infrastruktury, které umožňují elektronické poskytování síťových služeb, zpravidla po internetu, které zajišťují transevropské interoperabilní služby společného zájmu pro občany, podniky nebo vlády a které jsou tvořeny platformami hlavních služeb a obecnými službami."@cs,
    "These are infrastructures that allow the electronic provision of network services, generally via the Internet, which provide trans-European interoperable services of common interest to citizens, businesses or governments, and which consist of core service platforms and universal services."@en,
    "is a collection of cross-sectorial infrastructure services and components. They are decoupled from the business which a specific interoperable solution implements. They can be re-used with no or very minor changes by other interoperable solutions or in different policy contexts. [CEF] [8]."@en;
  skos:inScheme g-sgov-european-interoperability-reference-architecture:glosář;
  skos:prefLabel "Digital Service Infrastructure"@en, "Infrastruktura digitálních služeb"@cs .

g-sgov-european-interoperability-reference-architecture-pojem:kalatog-datových-sad
  a skos:Concept;
  skos:inScheme g-sgov-european-interoperability-reference-architecture:glosář;
  skos:prefLabel "Data Set Catalogue"@en, "Kalatog datových sad"@cs .

g-sgov-european-interoperability-reference-architecture-pojem:katalog-datových-standardů
  a skos:Concept;
  skos:inScheme g-sgov-european-interoperability-reference-architecture:glosář;
  skos:prefLabel "Data Standard Catalogue"@en, "Katalog datových standardů"@cs .

g-sgov-european-interoperability-reference-architecture-pojem:katalog-legislativy
  a skos:Concept;
  skos:inScheme g-sgov-european-interoperability-reference-architecture:glosář;
  skos:prefLabel "Katalog legislativy"@cs, "Legislation Catalogue"@en .

g-sgov-european-interoperability-reference-architecture-pojem:katalog-veřejných-služeb
  a skos:Concept;
  skos:inScheme g-sgov-european-interoperability-reference-architecture:glosář;
  skos:prefLabel "Katalog veřejných služeb"@cs, "Public Service Catalog"@en .

g-sgov-european-interoperability-reference-architecture-pojem:m2m-rozhraní a skos:Concept;
  skos:definition "is a description of a boundary between a system and other systems, usually including the mechanisms by which information is transferred."@en;
  skos:inScheme g-sgov-european-interoperability-reference-architecture:glosář;
  skos:prefLabel "M2M rozhraní"@cs, "Machine to Machine Interface"@en .

g-sgov-european-interoperability-reference-architecture-pojem:model-dodávky-služeb
  a skos:Concept;
  skos:inScheme g-sgov-european-interoperability-reference-architecture:glosář;
  skos:prefLabel "Model dodávky služeb"@cs, "Service Delivery Model"@en .

g-sgov-european-interoperability-reference-architecture-pojem:nástroj-formulace-a-zavedení-politiky
  a skos:Concept;
  skos:inScheme g-sgov-european-interoperability-reference-architecture:glosář;
  skos:prefLabel "Nástroj formulace a zavedení politiky"@cs, "Public Policy Formulation and Implementation Instruments"@en .

g-sgov-european-interoperability-reference-architecture-pojem:občan a skos:Concept;
  skos:inScheme g-sgov-european-interoperability-reference-architecture:glosář;
  skos:prefLabel "Citizen"@en, "Občan"@cs .

g-sgov-european-interoperability-reference-architecture-pojem:organizační-předpoklad-interoperability
  a skos:Concept;
  skos:inScheme g-sgov-european-interoperability-reference-architecture:glosář;
  skos:prefLabel "Organizational Interoperability Enabler"@en, "Organizační předpoklad interoperability"@cs .

g-sgov-european-interoperability-reference-architecture-pojem:podpůrné-hledisko-specifikace-interoperability
  a skos:Concept;
  skos:inScheme g-sgov-european-interoperability-reference-architecture:glosář;
  skos:prefLabel "Interoperability specification underpinning view"@en, "Podpůrné hledisko specifikace interoperability"@cs .

g-sgov-european-interoperability-reference-architecture-pojem:poskytovatel-veřejné-služby
  a skos:Concept;
  skos:inScheme g-sgov-european-interoperability-reference-architecture:glosář;
  skos:prefLabel "Poskytovatel veřejné služby"@cs, "Public Service Provider"@en .

g-sgov-european-interoperability-reference-architecture-pojem:prostředek---reprezentace
  a skos:Concept;
  skos:definition "is the means through which the other building blocks (data, data sets, etc.) are physically realised. This can be done through modelling notations, schemas and other resources."@en;
  skos:inScheme g-sgov-european-interoperability-reference-architecture:glosář;
  skos:prefLabel "Prostředek / reprezentace"@cs, "Representation"@en .

g-sgov-european-interoperability-reference-architecture-pojem:předpoklad-rozvoje-politiky
  a skos:Concept;
  skos:inScheme g-sgov-european-interoperability-reference-architecture:glosář;
  skos:prefLabel "Public Policy Development Enabler"@en, "Předpoklad rozvoje politiky"@cs .

g-sgov-european-interoperability-reference-architecture-pojem:schopnost a skos:Concept;
  skos:definition "is the expression or the articulation of the capacity, materials and expertise an organization needs in order to perform core functions. Enterprise architects use business capabilities to illustrate the over-arching needs of the business in order to better strategize IT solutions that meet those business needs."@en;
  skos:inScheme g-sgov-european-interoperability-reference-architecture:glosář;
  skos:prefLabel "Business Capability"@en, "Schopnost"@cs .

g-sgov-european-interoperability-reference-architecture-pojem:služba-choreografie-služeb
  a skos:Concept;
  skos:definition """is the interplay among groups of services which, in turn, make up a larger, composite service, or which interact across organisational boundaries in order to obtain and process information. 
A choreography's role specifies the expected messaging behavior of the participants that will play it in terms of the sequencing and timing of the messages that they can consume and produce.[Wiki]
Like in a dancing stage, every dancer knows exactly what to do, and looks to all the other dancers involved in the process, to synchronize his steps.
A single remote system knows what to do and also what other systems to call after he ends his processing."""@en;
  skos:inScheme g-sgov-european-interoperability-reference-architecture:glosář;
  skos:prefLabel "Choreohraphy Service"@en, "Služba choreografie (služeb)"@cs .

g-sgov-european-interoperability-reference-architecture-pojem:služba-orchestrace-služeb
  a skos:Concept;
  skos:definition """Orchestration identifies a sets of transactions involving use of other services and functionalities, according to business rules embodied in one or more documented business processes, with the ultimate goal of performing or providing some other value-added function or service. The Orchestration Service executes all the required transactions and routes the inputs and outputs of processes according to rules described in a standard language (i.e. BPEL).
Like in an orchestra, there's a man (the director) that says to all the musicians what to do. They're therefore synchronized by following the direction of one person.
In practice when orchestration is in place, a central system says to some remote systems what to do."""@en;
  skos:inScheme g-sgov-european-interoperability-reference-architecture:glosář;
  skos:prefLabel "Orchestration Service"@en, "Služba orchestrace (služeb)"@cs .

g-sgov-european-interoperability-reference-architecture-pojem:služby-infrastruktury-pro-hosting-a-síťovou-komunikaci
  a skos:Concept;
  skos:definition "is a collection of services for hosting Interoperable European Solutions and provides the necessary networks for operating these solutions."@en;
  skos:inScheme g-sgov-european-interoperability-reference-architecture:glosář;
  skos:prefLabel "Hosting and Networking Infrastructure Service"@en, "Služby infrastruktury pro hosting a síťovou komunikaci"@cs .

g-sgov-european-interoperability-reference-architecture-pojem:specifikace-byznys-interoperability
  a skos:Concept;
  skos:definition "defines the interoperability aspects for a [Public Service Catalogue] (contents and the catalogue as a whole) and is described in an [Interoperability Agreement]."@en;
  skos:inScheme g-sgov-european-interoperability-reference-architecture:glosář;
  skos:prefLabel "Organizational Interoperability Specification"@en, "Specifikace byznys interoperability"@cs .

g-sgov-european-interoperability-reference-architecture-pojem:specifikace-právní-interoperability
  a skos:Concept;
  skos:definition "defines the interoperability aspects for a [Legislation Catalogue] (contents and the catalogue as a whole) and is associated to [Public Policy Formulation and Implement Instrument]. "@en;
  skos:inScheme g-sgov-european-interoperability-reference-architecture:glosář;
  skos:prefLabel "Legal Interoperability Specification"@en, "Specifikace právní interoperability"@cs .

g-sgov-european-interoperability-reference-architecture-pojem:specifikace-sémantické-interoperability
  a skos:Concept;
  skos:definition "defines the interoperability aspects for a [Data Set Catalogue] (contents and the catalogue as a whole) and/or [Data Standards Catalogue] (contents and the catalogue as a whole)."@en;
  skos:inScheme g-sgov-european-interoperability-reference-architecture:glosář;
  skos:prefLabel "Semantic Interoperability Specification"@en, "Specifikace sémantické interoperability"@cs .

g-sgov-european-interoperability-reference-architecture-pojem:specifikace-technologické-interoperability
  a skos:Concept;
  skos:definition "Is describing aspects of the underlying system. The [Service Registry Component] provides a mechanism to register technical services within a catalogue to be discovered by others."@en;
  skos:inScheme g-sgov-european-interoperability-reference-architecture:glosář;
  skos:prefLabel "Specifikace technologické interoperability"@cs, "Technology Interoperabilty Specification"@en .

g-sgov-european-interoperability-reference-architecture-pojem:spotřebitel-veřejné-služby
  a skos:Concept;
  skos:inScheme g-sgov-european-interoperability-reference-architecture:glosář;
  skos:prefLabel "Public Service Consumer"@en, "Spotřebitel veřejné služby"@cs .

g-sgov-european-interoperability-reference-architecture-pojem:uživatelské-rozhraní
  a skos:Concept;
  skos:definition "is a specific interface between the human users of an IT system and the programs providing screen or printed results. It is frequently regarded as a dedicated set of programs, separate from those which extract and process data."@en;
  skos:inScheme g-sgov-european-interoperability-reference-architecture:glosář;
  skos:prefLabel "Human Interface"@en, "Uživatelské rozhraní"@cs .

g-sgov-european-interoperability-reference-architecture-pojem:veřejná-politika a skos:Concept;
  skos:definition "is the whole of actions under a policy domain taken by a public authority to bring about social change in the medium and long term. It is based on certain values and objectives and is implemented using a variety of methods. It applies on the territory within which the authority is authorised to act [Eurovoc]"@en;
  skos:inScheme g-sgov-european-interoperability-reference-architecture:glosář;
  skos:prefLabel "Public Policy"@en, "Veřejná politika"@cs .

g-sgov-european-interoperability-reference-architecture-pojem:veřejná-služba a skos:Concept;
  skos:definition "is an economic activity that public authorities identify as being of particular importance to citizens, businesses and public administrations and that would not be supplied (or would be supplied under different conditions) if there were no public intervention [DG Competition]. A public service is also the capacity to carry out a procedure and exists whether it is used or not. It is a set of deeds and acts performed by or on behalf of a public agency for the benefit of a citizen, a business or another public agency [CoreVoc]. A Public Service is considered also based on the commitment to provide it by its provider, regardless of whether or not it is actively being offered."@en;
  skos:inScheme g-sgov-european-interoperability-reference-architecture:glosář;
  skos:prefLabel "Public Service"@en, "Veřejná služba"@cs .

g-sgov-european-interoperability-reference-architecture-pojem:výměna-informací a skos:Concept;
  skos:definition "is an interaction between two or more public administrations, businesses or citizens. [ISO15000-5, UN/CEFACT CCTS]."@en;
  skos:inScheme g-sgov-european-interoperability-reference-architecture:glosář;
  skos:prefLabel "Business Information Exchange"@en, "Výměna informací"@cs .

g-sgov-european-interoperability-reference-architecture-pojem:zprostředkovatel-dodávky-veřejné-služby
  a skos:Concept;
  skos:inScheme g-sgov-european-interoperability-reference-architecture:glosář;
  skos:prefLabel "Public Service Delivery Agent"@en, "Zprostředkovatel dodávky veřejné služby"@cs .
