@prefix a-popis-dat-pojem: <http://onto.fel.cvut.cz/ontologies/slovník/agendový/popis-dat/pojem/> .
@prefix dcterms: <http://purl.org/dc/terms/> .
@prefix g-sgov-iso-iec-270372012-10-15: <https://slovník.gov.cz/generický/iso-iec-270372012-10-15/> .
@prefix g-sgov-iso-iec-270372012-10-15-pojem: <https://slovník.gov.cz/generický/iso-iec-270372012-10-15/pojem/> .
@prefix rdf: <http://www.w3.org/1999/02/22-rdf-syntax-ns#> .
@prefix skos: <http://www.w3.org/2004/02/skos/core#> .
@prefix xsd: <http://www.w3.org/2001/XMLSchema#> .

g-sgov-iso-iec-270372012-10-15:glosář a a-popis-dat-pojem:glosář, skos:ConceptScheme;
  dcterms:title "ISO/IEC 27037:2012-10-15"@cs;
  skos:hasTopConcept g-sgov-iso-iec-270372012-10-15-pojem:digitální-evidence, g-sgov-iso-iec-270372012-10-15-pojem:digitální-paměťové-médium,
    g-sgov-iso-iec-270372012-10-15-pojem:systémový-čas, g-sgov-iso-iec-270372012-10-15-pojem:zařízení-na-uchovávání-důkazů,
    g-sgov-iso-iec-270372012-10-15-pojem:časové-razítko .

g-sgov-iso-iec-270372012-10-15-pojem:digitální-evidence a skos:Concept;
  dcterms:source "3.5";
  skos:definition "information or data, stored or transmitted in binary form that may be relied on as evidence"@en;
  skos:inScheme g-sgov-iso-iec-270372012-10-15:glosář;
  skos:prefLabel "Digital Evidence"@en, "Digitální evidence"@cs .

g-sgov-iso-iec-270372012-10-15-pojem:digitální-paměťové-médium a skos:Concept;
  dcterms:source "3.9";
  skos:definition """device on which digital data may be recorded
[Adapted from ISO/IEC 10027:1990]"""@en;
  skos:inScheme g-sgov-iso-iec-270372012-10-15:glosář;
  skos:prefLabel "Digital Storage Medium"@en, "Digitální paměťové médium"@cs .

g-sgov-iso-iec-270372012-10-15-pojem:časové-razítko a skos:Concept;
  dcterms:source "3.22";
  skos:definition """time variant parameter which denotes a point in time with respect to a common time reference
[ISO/IEC 11770-1:1996]"""@en;
  skos:inScheme g-sgov-iso-iec-270372012-10-15:glosář;
  skos:prefLabel "Timestamp"@en, "Časové razítko"@cs .

g-sgov-iso-iec-270372012-10-15-pojem:systémový-čas a skos:Concept;
  dcterms:source "3.20";
  skos:definition "time generated by the system clock and used by the operating system, not the time computed by the operating system"@en;
  skos:inScheme g-sgov-iso-iec-270372012-10-15:glosář;
  skos:prefLabel "System Time"@en, "Systémový čas"@cs .

g-sgov-iso-iec-270372012-10-15-pojem:zařízení-na-uchovávání-důkazů a skos:Concept;
  dcterms:source "3.10";
  skos:definition """secure environment or a location where collected or acquired evidence is stored
NOTE　An evidence preservation facility should not be exposed to magnetic fields, dust, vibration, moisture or any other environmental elements (such as extreme temperature or humidity) that may damage the potential digital evidence within the facility."""@en;
  skos:inScheme g-sgov-iso-iec-270372012-10-15:glosář;
  skos:prefLabel "Evidence Preservation Facility"@en, "Zařízení na uchovávání důkazů"@cs .
