@prefix a-popis-dat-pojem: <http://onto.fel.cvut.cz/ontologies/slovník/agendový/popis-dat/pojem/> .
@prefix dcterms: <http://purl.org/dc/terms/> .
@prefix g-sgov-iso-iec-270392015-02-15-iso-iec-270392016-05-01: <https://slovník.gov.cz/generický/iso-iec-270392015-02-15-iso-iec-270392016-05-01/> .
@prefix g-sgov-iso-iec-270392015-02-15-iso-iec-270392016-05-01-pojem: <https://slovník.gov.cz/generický/iso-iec-270392015-02-15-iso-iec-270392016-05-01/pojem/> .
@prefix rdf: <http://www.w3.org/1999/02/22-rdf-syntax-ns#> .
@prefix skos: <http://www.w3.org/2004/02/skos/core#> .
@prefix xsd: <http://www.w3.org/2001/XMLSchema#> .

g-sgov-iso-iec-270392015-02-15-iso-iec-270392016-05-01:glosář a a-popis-dat-pojem:glosář,
    skos:ConceptScheme;
  dcterms:title """ISO/IEC 27039:2015-02-15
ISO/IEC 27039:2016-05-01"""@cs;
  skos:hasTopConcept g-sgov-iso-iec-270392015-02-15-iso-iec-270392016-05-01-pojem:detekce-vniknutí,
    g-sgov-iso-iec-270392015-02-15-iso-iec-270392016-05-01-pojem:dohoda-ujednání-o-úrovni-služeb,
    g-sgov-iso-iec-270392015-02-15-iso-iec-270392016-05-01-pojem:průnik, g-sgov-iso-iec-270392015-02-15-iso-iec-270392016-05-01-pojem:senzor,
    g-sgov-iso-iec-270392015-02-15-iso-iec-270392016-05-01-pojem:server, g-sgov-iso-iec-270392015-02-15-iso-iec-270392016-05-01-pojem:trojský-kůň,
    g-sgov-iso-iec-270392015-02-15-iso-iec-270392016-05-01-pojem:vetřelec, g-sgov-iso-iec-270392015-02-15-iso-iec-270392016-05-01-pojem:vir,
    g-sgov-iso-iec-270392015-02-15-iso-iec-270392016-05-01-pojem:využití, g-sgov-iso-iec-270392015-02-15-iso-iec-270392016-05-01-pojem:zajištění .

g-sgov-iso-iec-270392015-02-15-iso-iec-270392016-05-01-pojem:detekce-vniknutí a skos:Concept;
  dcterms:source "2.17";
  skos:definition "formal process of detecting intrusions, generally characterized by gathering knowledge about abnormal usage patterns, as well as what, how, and which vulnerability has been exploited to include how and when it occurred"@en;
  skos:inScheme g-sgov-iso-iec-270392015-02-15-iso-iec-270392016-05-01:glosář;
  skos:prefLabel "Detekce vniknutí"@cs, "Intrusion detection"@en .

g-sgov-iso-iec-270392015-02-15-iso-iec-270392016-05-01-pojem:dohoda-ujednání-o-úrovni-služeb
  a skos:Concept;
  dcterms:source "2.27";
  skos:definition "document that defines the technical support or business performance objectives including measures for performance and consequences for failure the provider of a service can provide its clients"@en;
  skos:inScheme g-sgov-iso-iec-270392015-02-15-iso-iec-270392016-05-01:glosář;
  skos:prefLabel "Dohoda (ujednání) o úrovni služeb"@cs, "Service Level Agreement"@en .

g-sgov-iso-iec-270392015-02-15-iso-iec-270392016-05-01-pojem:průnik a skos:Concept;
  dcterms:source "2.21";
  skos:definition "unauthorized act of bypassing the security mechanisms of information systems"@en;
  skos:inScheme g-sgov-iso-iec-270392015-02-15-iso-iec-270392016-05-01:glosář;
  skos:prefLabel "Penetration"@en, "Průnik"@cs .

g-sgov-iso-iec-270392015-02-15-iso-iec-270392016-05-01-pojem:senzor a skos:Concept;
  dcterms:source "2.28";
  skos:definition """component/agent of IDPS which collects event data from information systems or a network under observation
Note 1 to entry: Also referred to as a monitor."""@en;
  skos:inScheme g-sgov-iso-iec-270392015-02-15-iso-iec-270392016-05-01:glosář;
  skos:prefLabel "Sensor"@en, "Senzor"@cs .

g-sgov-iso-iec-270392015-02-15-iso-iec-270392016-05-01-pojem:server a skos:Concept;
  dcterms:source "2.26";
  skos:definition "computer system or program that provides services to other computers"@en;
  skos:inScheme g-sgov-iso-iec-270392015-02-15-iso-iec-270392016-05-01:glosář;
  skos:prefLabel "Server"@cs, "Server"@en .

g-sgov-iso-iec-270392015-02-15-iso-iec-270392016-05-01-pojem:trojský-kůň a skos:Concept;
  dcterms:source "2.32";
  skos:definition "malicious program that masquerades as a benign application"@en;
  skos:inScheme g-sgov-iso-iec-270392015-02-15-iso-iec-270392016-05-01:glosář;
  skos:prefLabel "Trojan Horse"@en, "Trojský kůň"@cs .

g-sgov-iso-iec-270392015-02-15-iso-iec-270392016-05-01-pojem:vetřelec a skos:Concept;
  dcterms:source "2.15";
  skos:definition "individual who is conducting, or has conducted, an intrusion or attack against a victim’s host, site, network, or organization"@en;
  skos:inScheme g-sgov-iso-iec-270392015-02-15-iso-iec-270392016-05-01:glosář;
  skos:prefLabel "Intruder"@en, "Vetřelec"@cs .

g-sgov-iso-iec-270392015-02-15-iso-iec-270392016-05-01-pojem:vir a skos:Concept;
  dcterms:source "2.33";
  skos:definition "type of malware which is software designed with malicious intent containing features or capabilities that can potentially cause harm, directly or indirectly, to the user and/or the user’s system"@en;
  skos:inScheme g-sgov-iso-iec-270392015-02-15-iso-iec-270392016-05-01:glosář;
  skos:prefLabel "Vir"@cs, "Virus"@en .

g-sgov-iso-iec-270392015-02-15-iso-iec-270392016-05-01-pojem:využití a skos:Concept;
  dcterms:source "2.9";
  skos:definition "defined way to breach the security of information systems through vulnerability"@en;
  skos:inScheme g-sgov-iso-iec-270392015-02-15-iso-iec-270392016-05-01:glosář;
  skos:prefLabel "Exploit"@en, "Využití"@cs .

g-sgov-iso-iec-270392015-02-15-iso-iec-270392016-05-01-pojem:zajištění a skos:Concept;
  dcterms:source "2.22";
  skos:definition "process of loading the correct software, security policy, and configuration data for information technology (IT) devices"@en;
  skos:inScheme g-sgov-iso-iec-270392015-02-15-iso-iec-270392016-05-01:glosář;
  skos:prefLabel "Provisioning"@en, "Zajištění"@cs .
