@prefix a-popis-dat-pojem: <http://onto.fel.cvut.cz/ontologies/slovník/agendový/popis-dat/pojem/> .
@prefix dcterms: <http://purl.org/dc/terms/> .
@prefix g-sgov-iso-iec-15408-12014-01-15: <https://slovník.gov.cz/generický/iso-iec-15408-12014-01-15/> .
@prefix g-sgov-iso-iec-15408-12014-01-15-pojem: <https://slovník.gov.cz/generický/iso-iec-15408-12014-01-15/pojem/> .
@prefix rdf: <http://www.w3.org/1999/02/22-rdf-syntax-ns#> .
@prefix skos: <http://www.w3.org/2004/02/skos/core#> .
@prefix xsd: <http://www.w3.org/2001/XMLSchema#> .

g-sgov-iso-iec-15408-12014-01-15:glosář a a-popis-dat-pojem:glosář, skos:ConceptScheme;
  dcterms:title "ISO/IEC 15408-1:2014-01-15"@cs;
  skos:hasTopConcept g-sgov-iso-iec-15408-12014-01-15-pojem:administrátor, g-sgov-iso-iec-15408-12014-01-15-pojem:autorizovaný-uživatel,
    g-sgov-iso-iec-15408-12014-01-15-pojem:potenciál-útoku, g-sgov-iso-iec-15408-12014-01-15-pojem:rozhraní,
    g-sgov-iso-iec-15408-12014-01-15-pojem:softwareové-inženýrství, g-sgov-iso-iec-15408-12014-01-15-pojem:závislost .

g-sgov-iso-iec-15408-12014-01-15-pojem:administrátor a skos:Concept;
  dcterms:source "3.2.1";
  skos:definition """entity that has a level of trust with respect to all policies implemented by the TSF
NOTE　Not all PPs or STs assume the same level of trust for administrators. Typically administrators are assumed to adhere at all times to the policies in the ST of the TOE. Some of these policies may be related to the functionality of the TOE, others may be related to the operational environment."""@en;
  skos:inScheme g-sgov-iso-iec-15408-12014-01-15:glosář;
  skos:prefLabel "Administrator"@en, "Administrátor"@cs .

g-sgov-iso-iec-15408-12014-01-15-pojem:autorizovaný-uživatel a skos:Concept;
  dcterms:source "3.1.8";
  skos:definition "TOE user who may, in accordance with the SFRs, perform an operation"@en;
  skos:inScheme g-sgov-iso-iec-15408-12014-01-15:glosář;
  skos:prefLabel "Autorizovaný uživatel"@cs, "authorised user"@en .

g-sgov-iso-iec-15408-12014-01-15-pojem:potenciál-útoku a skos:Concept;
  dcterms:source "3.1.5";
  skos:definition "measure of the effort to be expended in attacking a TOE, expressed in terms of an attacker's expertise, resources and motivation"@en;
  skos:inScheme g-sgov-iso-iec-15408-12014-01-15:glosář;
  skos:prefLabel "Attack Potential"@en, "Potenciál útoku"@cs .

g-sgov-iso-iec-15408-12014-01-15-pojem:rozhraní a skos:Concept;
  dcterms:source "3.2.17";
  skos:definition "means of interaction with a component or module"@en, "zařízení, program nebo formát zajištující správnou komunikaci a přenos mezi odlišnými zařízeními nebo programy"@cs;
  skos:inScheme g-sgov-iso-iec-15408-12014-01-15:glosář;
  skos:prefLabel "Interface"@en, "Rozhraní "@cs .

g-sgov-iso-iec-15408-12014-01-15-pojem:softwareové-inženýrství a skos:Concept;
  dcterms:source "3.2.24";
  skos:definition """application of a systematic, disciplined, quantifiable approach to the development and maintenance of software; that is, the application of engineering to software
[IEEE Std 610.12-1990]
NOTE　As with engineering practices in general, some amount of judgement must be used in applying engineering principles. Many factors affect choices, not just the application of measures of modular decomposition, layering, and minimization. For example, a developer may design a system with future applications in mind that will not be implemented initially. The developer may choose to include some logic to handle these future applications without fully implementing them; further, the developer may include some calls to as-yet unimplemented modules, leaving call stubs. The developer's justification for such deviations from well-structured programs will have to be assessed using judgement, as well as the application of good software engineering discipline."""@en;
  skos:inScheme g-sgov-iso-iec-15408-12014-01-15:glosář;
  skos:prefLabel "Software Engineering"@en, "Softwareové inženýrství"@cs .

g-sgov-iso-iec-15408-12014-01-15-pojem:závislost a skos:Concept;
  dcterms:source "3.1.20";
  skos:definition "relationship between components such that if a requirement based on the depending component is included in a PP, ST or package, a requirement based on the component that is depended upon must normally also be included in the PP, ST or package"@en;
  skos:inScheme g-sgov-iso-iec-15408-12014-01-15:glosář;
  skos:prefLabel "Závislost"@cs, "dependency"@en .
